finished beta-reduction case of CPS-translation correctness
~3 admitted lemmas remaining.

theories/L4_deBruijn/simpleCPSAA.v
@@ -2,12 +2,12 @@
 (** coqide -R /path/to/SquiggleLazyEq SquiggleLazyEq 
 https://github.com/aa755/SquiggleLazyEq
 
-This file does NOT fully compile yet.
 *)
 
 (** CPS conversion for a language with nominal style variable bindings.
 We use the 
-SquiggleLazyEq library for generically defined substitution, alpha equality (and soon, a contextual equivalence)
+SquiggleLazyEq library for generically defined substitution, 
+alpha equality (and soon, a contextual computational equivalence)
 and several proofs about them.
 *)
 
@@ -20,6 +20,7 @@ Opaque N.sub.
 Lemma N_plus_minus:
   forall n:N, n > 0 -> (n - 1 + 1) = (n + 1 - 1).
 Proof.
+  intros.
   induction n using N.peano_ind; intros; lia.
 Qed.
 
@@ -187,6 +188,11 @@ Ltac if_split :=
     | [ |- context[if ?e then _ else _] ] => destruct e ; simpl ; try lia ; auto ; try subst
   end.
 
+Ltac if_splitH H := 
+  match type of H with
+    context[if ?e then _ else _] => destruct e
+  end.
+
 
 Class Substitute (v:Type) (t:Type) := { substitute : v -> NVar -> t -> t }.
 
@@ -236,96 +242,130 @@ Inductive eval : NTerm -> NTerm -> Prop :=
                   select n es = Some e' ->
                   eval (Proj_e e n) (e'{xf:=Fix_e xf es}).
 
-(** Evaluation preserves closedness.*)
-Lemma eval_preserves_closed :
-  forall e v, eval e v ->  closed e -> closed v.
+(** will be used in [eval_reduces_fvars] and cps_cvt_corr *)
+Lemma subsetv_step_app: forall x e1' v2,
+  subsetv (free_vars (e1' {x := v2})) (free_vars (App_e (Lam_e x e1') v2)).
+Proof.
+  intros. simpl. autorewrite with list core. unfold subst.
+  rewrite eqsetv_free_vars_disjoint.
+  apply subsetv_prop.
+  intros ? Hc.
+  rewrite in_app_iff in *.
+  simpl in Hc.
+  dorn Hc;[left; firstorder|right].
+  rewrite memvar_dmemvar in Hc.
+  if_splitH Hc; simpl in Hc; autorewrite with list in *;firstorder.
+Qed.
+
+Lemma eval_reduces_fvars :
+  forall e v, eval e v ->  subset (free_vars v) (free_vars e).
 Proof.
   intros ? ? He. unfold closed. induction He; try auto;
   simpl in *;autorewrite with core list in *.
-  - intro Hc. 
-    apply app_eq_nil in Hc. repnd.
-    apply_clear IHHe1 in Hc0.
-    apply_clear IHHe2 in Hc.
-    apply IHHe3.
-    unfold subst.
-    rewrite fvars_lsubst1; auto.
-    intros  ? ? Hin. in_reasoning. inverts Hin. subst. auto.
+  (**Apply case*)
+  -
+    applyall subsetv_prop. unfold subset. apply subsetv_prop.
+    pose proof (subsetv_step_app x e1' v2) as H.
+    pose proof (subsetv_trans _ _ _ IHHe3 H).
+    clear H IHHe3. eapply subsetv_trans; eauto.
+    simpl. autorewrite with list core.
+    apply subsetvAppLR; firstorder.
 
   - rename H into Hl. rename H0 into H1i. rename H1 into H2i.
     change es  with (fst (es, vs)).
-    change vs  with (snd (es, vs)) at 2.
+    change vs  with (snd (es, vs)) at 1.
     apply combine_split in Hl.
     rewrite <- Hl.
     rewrite fst_split_as_map, snd_split_as_map.
     repeat rewrite flat_map_map.
     repeat rw flat_map_empty.
-    intros Hf ? Hin. specialize (Hf _ Hin). unfold compose in *. 
-    simpl in *. autorewrite with core list in *.
-    destruct a.
-    eauto.
+    unfold subset. setoid_rewrite in_flat_map. 
+    unfold compose. simpl.
+    intros ? Hin. exrepnd. eexists. split;[apply Hin1|].
+    autorewrite with list core in *.
+    firstorder.
 
-  - simpl. intros Hf. apply IHHe2.
-    unfold subst.
-    apply app_eq_nil in Hf.
-    rewrite fvars_lsubst1;[tauto|].
-    unfold closed. simpl.
-    intros ? ? Hin. dorn Hin;[| contradiction].
-    inverts Hin. tauto.
+  (**Let case; same as the Apply case*)
+  - simpl in IHHe2. intros ? Hc.
+    apply_clear IHHe2 in Hc. unfold subst in Hc.
+    rewrite eqsetv_free_vars_disjoint in Hc.
+    simpl in Hc.
+    rewrite in_app_iff in *.
+    apply or_comm.
+    simpl in Hc.
+    dorn Hc;[left; firstorder|right].
+    rewrite memvar_dmemvar in Hc.
+    if_splitH Hc; simpl in Hc; autorewrite with list in *;firstorder.
 
-  - intros Hf. apply_clear IHHe2.
+  - intros ? Hf. apply_clear IHHe2 in Hf.
     destruct e' as [lv nt].
-    apply app_eq_nil in Hf. repnd.
-    apply_clear IHHe1 in Hf0.
-    rewrite flat_map_map in Hf.
-    rw flat_map_empty in Hf.
+    unfold apply_bterm in Hf. simpl in Hf.
+    rewrite eqsetv_free_vars_disjoint in Hf.
     revert H. destFind; intro Hdf; [| discriminate].
     repnd.
-    apply_clear Hf in Heqsnl0. invertsn Hdf.
     destruct bss as [xxx brbt]. simpl in Hdf. subst.
     apply andb_true_iff, proj1,beq_nat_true in Heqsnl.
-    unfold compose in Heqsnl0. simpl in *.
-    apply closed_bt_implies; auto;[|rewrite <- Heqsnl;refl].
-    rewrite flat_map_map in Hf0.
-    rw flat_map_empty in Hf0.
-    cpx.
+    unfold compose in Heqsnl0. simpl in *. destruct brbt as [lvv ntt].
+    inverts Hdf. unfold num_bvars in Heqsnl. simpl in Heqsnl.
+    rewrite dom_sub_combine in Hf;[| auto]. clear Heqsn.
+    rewrite in_app_iff in *.
+    apply or_comm.
+    dorn Hf;[left|right].
+    + apply in_flat_map.
+      exists (bterm lv nt). repnd. split;[| assumption].
+      apply in_map_iff. eexists; eauto.
+    + apply IHHe1. apply in_sub_free_vars in Hf. exrepnd.
+      apply in_flat_map. exists (bterm [] t).
+      split;[| assumption]. apply in_map.
+      apply in_sub_keep_first in Hf0. apply proj1 in Hf0.
+      apply sub_find_some in Hf0. apply in_combine_r in Hf0.
+      assumption.
 
-- intros Hf. unfold subst.
-  apply_clear IHHe in Hf.
-  rewrite fvars_lsubst1.
-  + rewrite flat_map_map in Hf; simpl.
-    rw flat_map_empty in Hf. unfold compose in Hf. simpl in Hf.
-    apply select_in in H. eauto.
-  + intros ? ? Hin. in_reasoning. inverts Hin. apply Hf.
+- intros ? Hf. unfold subst.
+  apply_clear IHHe. unfold subst in Hf.
+  rewrite eqsetv_free_vars_disjoint in Hf.
+  rewrite flat_map_map. simpl in Hf.
+  rewrite in_app_iff in *.
+  dorn Hf. 
+  + unfold compose. repnd.
+    apply select_in in H. apply in_flat_map. eexists; split; eauto.
+  + rewrite memvar_dmemvar in Hf. 
+    if_splitH Hf; simpl in Hf; autorewrite with list in *;[|firstorder].
+    rewrite flat_map_map in Hf. assumption.
+Qed.
+
+(** Evaluation preserves closedness.*)
+Corollary eval_preserves_closed :
+  forall e v, eval e v ->  closed e -> closed v.
+Proof.
+  intros ? ?  He. unfold closed. intro Hc.
+  apply eval_reduces_fvars  in He.
+  rewrite Hc in He.
+  apply subsetv_prop in He.
+  apply subsetv_nil_r in He. assumption.
 Qed.
 
 (** Characterize values *)
 Inductive is_value : NTerm -> Prop :=
 | var_is_value : forall i, is_value (vterm i)
 | lam_is_value : forall x e, is_value (Lam_e x e)
-| con_is_value : forall d es, are_values es -> is_value (Con_e d es)
+| con_is_value : forall d es, (forall s, In s es -> is_value s) -> is_value (Con_e d es)
 (** Unlike in Nuprl, fix is a value.*)
-| fix_is_value : forall xf es, is_value (Fix_e xf es)
-with are_values : list NTerm -> Prop :=
-| nil_are_values : are_values nil
-| cons_are_values : forall e es, is_value e -> are_values es ->
-                                 are_values (e::es).
-Scheme is_value_ind2 := Induction for is_value Sort Prop
-with are_values_ind2 := Induction for are_values Sort Prop.
-Combined Scheme my_is_value_ind from is_value_ind2, are_values_ind2.
-Hint Constructors is_value are_values.
+| fix_is_value : forall xf es, is_value (Fix_e xf es).
 
-(** Show that evaluation always yields a value. 
+(** Show that evaluation always yields a value. *)
 Lemma eval_yields_value' :
-  (forall e v, eval e v -> is_value v) /\
-  (forall es vs, evals es vs -> are_values vs).
+  (forall e v, eval e v -> is_value v).
 Proof.
-  apply my_eval_ind ; simpl ; intros ; auto ; try constructor ; auto.
-Qed.
-*)
+  intros ? ? He ; induction He; simpl ; intros ; 
+  auto ; try constructor ; auto.
+(* easy *)
+Admitted.
+
 
 Lemma eval_yields_value e v : eval e v -> is_value v.
-Admitted.
-Hint Resolve eval_yields_value.
+Abort.
+(*Hint Resolve eval_yields_value. *)
 
 
 (**********************)
@@ -436,8 +476,11 @@ Inductive eval_c : CTerm -> CTerm -> Prop :=
 | eval_Ret_c : forall x c v v',
                  eval_c (c {x := v}) v' -> 
                  eval_c (Ret_c (KLam_c x c) v) v'
+
+(** use simultaneous substitution? *)
+
 | eval_Call_c : forall xk x c v1 v2 v',
-                  eval_c (c {xk:=v1}{x:=v2}) v' -> 
+                  eval_c (c {x:=v2}{xk:=v1}) v' -> 
                   eval_c (Call_c (KLam_c xk (Lam_c x c)) v1 v2) v'
 | eval_Match_c : forall d vs bs c v',
                    find_branch d (List.length vs) bs = Some c ->
@@ -453,19 +496,21 @@ Hint Constructors eval_c.
 
 (** Useful for rewriting. *)
 Lemma eval_ret :
-  forall x c v v', eval_c (Ret_c (KLam_c x c) v) v' <-> eval_c (c{x := v}) v'.
+  forall x c v v', eval_c (Ret_c (KLam_c x c) v) v' 
+  <-> eval_c (c{x := v}) v'.
 Proof.
   intros. split ; intro. inversion H. subst ; auto. constructor ; auto.
 Qed.
 
-(** Useful for rewriting. 
-Lemma eval_call :
-  forall c v1 v2 v',
-    eval_c (Call_c (Lam_c c) v1 v2) v' <-> eval_c (c{0:=v1}{0:=v2}) v'.
+(** Useful for rewriting. *)
+Lemma eval_call : forall xk x c v1 v2 v',
+   eval_c (Call_c (KLam_c xk (Lam_c x c)) v1 v2) v'
+  <-> eval_c (c {x:=v2}{xk:=v1}) v'.
 Proof.
-  intros ; split ; intro. inversion H ; subst ; auto. constructor ; auto.
+  intros ; split ; intro; inversion H ; subst ; auto.
 Qed.
 
+(*
 (** Useful for rewriting. *)
 Lemma eval_match :
   forall d vs bs v' c,
@@ -519,6 +564,11 @@ Fixpoint is_valueb (e:NTerm) : bool :=
       end
    end.
 
+Lemma is_valueb_corr :
+  (forall e, is_valueb e = true <-> is_value e).
+Proof.
+Admitted.
+
 
 (*
 Definition are_valuesb := are_valuesb' is_valueb.
@@ -543,11 +593,6 @@ Hint Rewrite are_valuesb_corr.
 Hint Resolve is_valueb_corr.
 Hint Resolve are_valuesb_corr.
 
-Fixpoint list_to_indices (es:list exp) : list val_c :=
-  match es with
-    | nil => nil
-    | e::es => (KVar_c (N.of_nat (List.length es)))::(list_to_indices es)
-  end.
 *)
 (** The inner, naive CBV CPS translation.  This introduces a lot of 
     administrative reductions, but simple things first.  Importantly,
@@ -556,90 +601,93 @@ Fixpoint list_to_indices (es:list exp) : list val_c :=
     [cps_cvt(e{x:=v}) = (cps_cvt e){x:=(cps_vt_val v)}].
  *)
  
-Notation "λ x . y" := (Lam_c x y) (at level 100).
-Notation "λ' x . y" := (KLam_c x y) (at level 100).
 Section CPS_CVT.
-  (* recursive call below *)
-  Variable cps_cvt : NTerm -> CTerm (*val_c *).
-  
-  Definition cps_cvt_bterm (b:BTerm) : CBTerm :=
+(** these are ALL vars, not just the free vars, of the top level term being converted*)
+(** recursive call below *)
+  Variable cps_cvt : (list NVar) -> NTerm -> CTerm (*val_c *).
+
+(*  
+  Definition cps_cvt_bterm  (fve : list NVar) (b:BTerm) : CBTerm :=
   match b with
   | bterm vars nt => bterm vars (cps_cvt nt)
   end.
+*)
 
-  (** the KLam_c was manually added. unlike now, fix previously implicitly bound var*)
-  Definition cps_cvt_fn_list' (es: list BTerm) : list CBTerm :=
+  (** the KLam_c was manually added. unlike now, Fix_c previously implicitly bound a var*)
+  Definition cps_cvt_fn_list' (fve : list NVar) (es: list BTerm) : list CBTerm :=
     map (fun b => 
             let e := get_nt b in
-            let vars := get_vars b in 
-            let kv := fresh_var (free_vars e) in 
-                    bterm vars (KLam_c kv (Ret_c (cps_cvt e) (vterm kv))) ) es.
+            let vars := get_vars b in
+            let kv := fresh_var (vars ++ fve) in 
+                    bterm vars (KLam_c kv (Ret_c (cps_cvt (vars ++ fve) e) (vterm kv))) ) es.
 
-  Fixpoint cps_cvt_val' (e:NTerm) : CTerm :=
+  Fixpoint cps_cvt_val'(fve : list NVar) (e:NTerm) : CTerm :=
     match e with
       | vterm n => vterm n
       | terms.oterm (opid.Can NLambda) [bterm [x] b] => 
-          let kv := fresh_var (free_vars b) in
-             KLam_c kv (Lam_c x (Ret_c (cps_cvt b) (vterm kv)))
+          let fvee := (x::fve) in
+          let kv := fresh_var fvee in
+             KLam_c kv (Lam_c x (Ret_c (cps_cvt fvee b) (vterm kv)))
       | terms.oterm (opid.Can (NDCon d _)) lb => 
-            Con_c d (List.map (cps_cvt_val' ∘ get_nt) lb)
+            Con_c d (List.map ((cps_cvt_val' fve) ∘ get_nt) lb)
       | terms.oterm (opid.Can (NFix nargs)) lb =>
           terms.oterm (CCan (CFix nargs))
-             (cps_cvt_fn_list' lb)
+             (cps_cvt_fn_list' fve lb)
       | _ => vterm nvarx (* impossible *)
     end.
 
-  Fixpoint cps_cvts' (vs: list NVar )(es:list BTerm) (c:CTerm) :  CTerm :=
+  Fixpoint cps_cvts' (fve : list NVar) (vs: list NVar )(es:list BTerm) (c:CTerm) :  CTerm :=
     match es with
       | nil => c
       | (bterm _ e)::es => 
         match vs with
-        | [] => Ret_c (cps_cvt e) (KLam_c nvarx (cps_cvts' [] es c)) (* impossible *)
-        | kvh :: kvt => Ret_c (cps_cvt e) (KLam_c kvh (cps_cvts' kvt es c))
+        | [] => Ret_c (cps_cvt fve e) (KLam_c nvarx (cps_cvts' fve [] es c)) (* impossible *)
+        | kvh :: kvt => Ret_c (cps_cvt fve e) (KLam_c kvh (cps_cvts' fve kvt es c))
         end
     end.
 
 
-  Definition cps_cvt_branch' (kv : NVar) (bt: BTerm) : CBTerm :=
+  Definition cps_cvt_branch' (fve : list NVar) (kv : NVar) (bt: BTerm) : CBTerm :=
     match bt with
     | bterm vars nt =>
-        (bterm vars (Ret_c (cps_cvt nt) (vterm kv)))
+        (bterm vars (Ret_c (cps_cvt (vars ++ fve) nt) (vterm kv)))
     end.
 
- Definition cps_cvt_branches' (kv : NVar) : (list BTerm) ->
+ Definition cps_cvt_branches' (fve : list NVar) (kv : NVar) : (list BTerm) ->
     list CBTerm :=
-  List.map (cps_cvt_branch' kv).
-    
+  List.map (cps_cvt_branch' fve kv).
 
 End CPS_CVT.
 
-(** make a wrapper that precomputes fve and passes to this function.  We dont want to do the fvar computation
-recursively*)
-Fixpoint cps_cvt (e:NTerm) : CTerm :=
-  let fve := free_vars e in (* the var library can have a way to compress a list of vars to a range, and have an alternate more efficient free vars function*)
-  if is_valueb e then let kv := fresh_var fve in KLam_c kv (Ret_c (vterm kv) (cps_cvt_val' cps_cvt e)) else
+Section CPSFvars.
+
+
+Fixpoint cps_cvt_aux (fve : list NVar) (e:NTerm) : CTerm :=
+  if is_valueb e 
+  then let kv := fresh_var fve in KLam_c kv (Ret_c (vterm kv) (cps_cvt_val' cps_cvt_aux fve e)) 
+    else
   match e with
     | terms.oterm (opid.NCan NApply) [bterm [] e1; bterm [] e2] => 
       (* cont \k.(ret [e1] (cont \v1.(ret [e2] (cont \v2.call v1 k v2)))) *)
       let kvars := projT1 (fresh_vars 3 fve) in 
       let k := nth 0 kvars nvarx in  
-      let v1 := nth 1 kvars nvarx in  
-      let v2 := nth 2 kvars nvarx in  
+      let k1 := nth 1 kvars nvarx in  
+      let k2 := nth 2 kvars nvarx in  
        KLam_c k 
-        (Ret_c (cps_cvt e1) (* e1 may not already be a lambda *)
-               (KLam_c v1 (Ret_c (cps_cvt e2)
-                                  (KLam_c v2 (Call_c (vterm v1) (vterm k) (vterm v2))))))
+        (Ret_c (cps_cvt_aux fve e1) (* e1 may not already be a lambda *)
+               (KLam_c k1 (Ret_c (cps_cvt_aux fve e2)
+                                  (KLam_c k2 (Call_c (vterm k1) (vterm k) (vterm k2))))))
     | terms.oterm (opid.Can (NDCon d nargs)) es => 
         let kvars := projT1 (fresh_vars (S (length es)) fve) in
         let k := hd nvarx kvars  in
-        KLam_c k (cps_cvts' cps_cvt (tail kvars) es (Ret_c (vterm k)
+        KLam_c k (cps_cvts' cps_cvt_aux fve (tail kvars) es (Ret_c (vterm k)
                                                           (Con_c d (map vterm kvars))))
     | terms.oterm (opid.NCan (NMatch brl)) ((bterm [] discriminee)::brr) => 
       let kvars := projT1 (fresh_vars 2 fve) in 
       let k := nth 0 kvars nvarx in
       let kd := nth 1 kvars nvarx in
-      let brrc :=  (bterm [] (vterm kd))::(cps_cvt_branches' cps_cvt k brr) in
-      KLam_c k (Ret_c (cps_cvt discriminee)
+      let brrc :=  (bterm [] (vterm kd))::(cps_cvt_branches' cps_cvt_aux fve k brr) in
+      KLam_c k (Ret_c (cps_cvt_aux fve discriminee)
                       (KLam_c kd 
                               (coterm (CNCan (CMatch brl)) brrc)))
     | terms.oterm (opid.NCan NLet) [bterm [] e1, bterm [x] e2] => 
@@ -648,26 +696,35 @@ Fixpoint cps_cvt (e:NTerm) : CTerm :=
       let kvars := projT1 (fresh_vars 3 fve) in 
       let k := nth 0 kvars nvarx in  
       let kvl := nth 1 kvars nvarx in  
-      let v2 := nth 2 kvars nvarx in  
-       KLam_c k (Ret_c (cps_cvt e2)
-                       (KLam_c v2 (Call_c (KLam_c kvl (Lam_c x (Ret_c (cps_cvt e2) (vterm kvl))))
+      let k2 := nth 2 kvars nvarx in  
+       KLam_c k (Ret_c (cps_cvt_aux (x::fve) e2)
+                       (KLam_c k2 (Call_c (KLam_c kvl (Lam_c x (Ret_c (cps_cvt_aux fve e1) (vterm kvl))))
                                           (vterm k) 
-                                          (vterm v2))))
+                                          (vterm k2))))
     | terms.oterm (opid.NCan (NProj i)) [bterm [] e] =>
       let kvars := projT1 (fresh_vars 2 fve) in 
       let k := nth 0 kvars nvarx in  
       let ke := nth 1 kvars nvarx in  
-        KLam_c k (Ret_c (cps_cvt e) 
+        KLam_c k (Ret_c (cps_cvt_aux fve e) 
                         (KLam_c ke (Proj_c (vterm ke) i (vterm k))))
     | _ => vterm nvarx (* impossible *)
   end.
+End CPSFvars.
 
-Definition cps_cvt_val := cps_cvt_val' cps_cvt.
+Definition cps_cvt (e:NTerm) : CTerm :=
+  let fve := free_vars e in (* the var library can have a way to compress a list of vars to a range, and have an alternate more efficient free vars function*)
+   cps_cvt_aux fve e.
+
+Definition cps_cvt_val (e:NTerm) : CTerm :=
+  let fve := free_vars e in 
+  cps_cvt_val' cps_cvt_aux fve e.
+(*
 Definition cps_cvts := cps_cvts' cps_cvt.
 Definition cps_cvt_vals := List.map cps_cvt_val.
 Definition cps_cvt_branch := cps_cvt_branch' cps_cvt.
 Definition cps_cvt_branches := cps_cvt_branches' cps_cvt.
 Definition cps_cvt_fn_list := cps_cvt_fn_list' cps_cvt.
+*)
 
 (** The top-level CPS translation.  We use [cont \x.Halt x] as the initial
     continuation. *)
@@ -727,2030 +784,308 @@ Eval vm_compute in eval_c_n 100 (cps_cvt_prog e9).
 Import List.
 Local Open Scope list_scope.
 
-(** Relationship between specialized CPS conversion for values
-    and the original translation. *)
-Lemma are_values_append : forall es1 es2, (are_values es1 /\ are_values es2) <->
-                                          are_values (es1 ++ es2).
-Proof.
-  induction es1 ; simpl ; intros ; split ; intro.
-  destruct H ; auto.
-  destruct H ; auto.
-  destruct H. inversion H. subst. constructor ; auto. rewrite <- IHes1. auto.
-  inversion H ; subst. rewrite <- IHes1 in H3. destruct H3. split ; auto.
-Qed.
-Hint Resolve are_values_append.
-  
-Lemma cps_val' :
-  (forall e, is_value e ->
-             cps_cvt e = Cont_c (Ret_c (KVar_c 0) (cps_cvt_val e))) /\
-  (forall es, are_values es ->
-     forall d es', are_values es' -> 
-        cps_cvt (Con_e d (es' ++ es)) =
-        Cont_c (Ret_c (KVar_c 0) (Con_c d (cps_cvt_vals (es' ++ es))))).
-Proof.
-  apply my_is_value_ind ; intros ; auto.
-  specialize (H d nil). replace ([] ++ es) with es in H ; auto.
-  repeat rewrite app_nil_r. simpl. fold are_valuesb.
-  rewrite (proj2 (are_valuesb_corr es') H). auto.
-  simpl. fold are_valuesb.
-  rewrite (proj2 (are_valuesb_corr (es' ++ (e::es)))) ; auto.
-  rewrite <- are_values_append. auto.
-Qed.
 
 Lemma cps_val :
-  forall v, is_value v -> cps_cvt v = Cont_c (Ret_c (KVar_c 0) (cps_cvt_val v)).
+  forall v:NTerm, 
+  closed v (* remove ?*)
+  ->
+  let k := fresh_var (free_vars v) in
+  is_value v -> cps_cvt v = (*only alpha equal?*) 
+    KLam_c k (Ret_c (vterm k) (cps_cvt_val v)).
 Proof.
-  intros. apply (proj1 cps_val'). auto.
-Qed.
-
-Lemma cps_vals :
-  forall vs d, are_values vs ->
-               cps_cvt (Con_e d vs) =
-               Cont_c (Ret_c (KVar_c 0) (Con_c d (cps_cvt_vals vs))).
-Proof.
-  intros.
-  specialize (proj2 cps_val' vs H d nil). simpl. auto.
-Qed.
-
-Lemma list_to_indices_wf :
-  forall es i j, vals_wf i (j + (N.of_nat (length es))) (list_to_indices es).
-Proof.
-  Opaque N.of_nat.
-  induction es ; simpl ; intros ; auto.
-  repeat constructor. lia. 
-  replace (j + (N.of_nat (S (length es)))) with ((1+j) + (N.of_nat (length es))) ; auto ; lia.
-Qed.
-
-(** The CPS translation produces continuation-closed terms. *)
-Lemma cps_kvar_closed' :
-  (forall i e, exp_wf i e ->
-     val_wf i 0 (cps_cvt e) /\ (is_value e -> val_wf i 0 (cps_cvt_val e))) /\
-  (forall i es, exps_wf i es ->
-     (forall j c, cps_wf i (j + (N.of_nat (length es))) c ->
-                  cps_wf i j (cps_cvts es c)) /\
-     (are_values es -> vals_wf i 0 (cps_cvt_vals es)) /\
-     (forall i', i = 2 + i' -> fn_list_wf i' 0 (cps_cvt_fn_list es))) /\
-  (forall i bs, branches_wf i bs -> cpsbranches_wf i 2 (cps_cvt_branches bs)).
-Proof.
-  apply my_exp_wf_ind ; simpl ; intros ; auto.
-  - repeat constructor ; auto.
-  - destruct H. repeat constructor.
-    apply (val_weaken _ _ _ H 0 2). apply (val_weaken _ _ _ H 0 1).
-  - destruct H. destruct H0. split.
-    + constructor. constructor.
-      apply (val_weaken _ _ _ H 0 1).
-      constructor. constructor.
-      apply (val_weaken _ _ _ H0 0 2).
-      repeat constructor.
-    + intros. inversion H3.
-  - destruct H. destruct H0. fold are_valuesb.
-    generalize (are_valuesb_corr es). intro.
-    destruct (are_valuesb es).
-    + specialize (H0 (proj1 H2 eq_refl)). repeat constructor; try auto.
-      * apply (vals_weaken _ _ _ H0 0 1). 
-    + split.
-      * constructor. apply H. repeat constructor. lia.
-        replace (1+0) with 1 ; auto.
-        eapply list_to_indices_wf.
-      * intros. inversion H3 ; subst.
-        destruct H2. specialize (H4 H5). discriminate.
-  - destruct H. split.
-    + repeat constructor ; auto. apply (val_weaken _ _ _ H 0 1).
-    + intro. inversion H2.
-  - destruct H ; destruct H0. split.
-    + repeat constructor ; auto.
-      apply (val_weaken _ _ _ H 0 1). apply (val_weaken _ _ _ H0 0 3).
-    + intro. inversion H3.
-  - destruct H. destruct H0. split. 
-    + repeat constructor ; auto.
-      specialize (H1 i eq_refl).
-      apply (fn_list_weaken _ _ _ H1 0 1). 
-    + intros. constructor. apply H1 ; auto.
-  - destruct H. split. repeat constructor ; auto.
-    apply (val_weaken _ _ _ H 0 1). intro. inversion H1.
-  - split ; auto. intros. rewrite (N.add_0_r) in H. auto.
-  - destruct H ; destruct H0. destruct H2. split ; intros.
-    + repeat constructor. 
-      * generalize (val_weaken _ _ _ H 0 j). rewrite (N.add_0_r). auto.
-      * apply H0.
-        replace (j + N.of_nat (S (length es)))
-        with (1 + j + N.of_nat (length es)) in H4 ; auto. lia.
-    + split ; intros.
-      * inversion H4 ; subst ; auto.
-      * subst. repeat constructor ; auto.
-        apply (val_weaken _ _ _ H 0 1).  
-  - constructor ; auto. destruct H. constructor.
-    + apply (val_weaken _ _ _ H 0 2). 
-    + constructor. lia.
-Qed.
-
-Lemma cps_kvar_closed i e : exp_wf i e -> val_wf i 0 (cps_cvt e).
-  intros. specialize (proj1 cps_kvar_closed' _ _ H). tauto.
-Qed.
-Lemma cps_val_kvar_closed i e : exp_wf i e -> is_value e -> val_wf i 0 (cps_cvt_val e).
-  intros. apply (proj2 (proj1 cps_kvar_closed' _ _ H) H0).
-Qed.
-Lemma cps_vals_kvar_closed i es : exps_wf i es -> are_values es -> vals_wf i 0 (cps_cvt_vals es).
-  intros.
-  apply (proj1 (proj2 (proj1 (proj2 cps_kvar_closed') i es H)) H0).
-Qed.
-Lemma cps_fn_list_closed i es : exps_wf (2 + i) es -> fn_list_wf i 0 (cps_cvt_fn_list es).
-  intros.
-  apply (proj2 (proj2 (proj1 (proj2 cps_kvar_closed') (2 + i) es H)) _ eq_refl).
-Qed.
-Lemma cps_branches_closed i bs : branches_wf i bs -> cpsbranches_wf i 2 (cps_cvt_branches bs).
-  intros. apply (proj2 (proj2 cps_kvar_closed') i bs H).
-Qed.
-Hint Resolve cps_kvar_closed cps_val_kvar_closed cps_vals_kvar_closed cps_fn_list_closed.
-
-(** Eliminate a continuation substitution when the index we are substituting
-    for is out of range. *)
-Lemma ksubst_closed :
-  (forall i j (e:cps), cps_wf i j e -> forall k, k >= j -> forall v, e[k:=v] = e) /\
-  (forall i j (w:val_c), val_wf i j w -> forall k, k >= j -> forall v, w[k:=v] = w) /\
-  (forall i j (ws:list val_c), vals_wf i j ws -> forall k, k >= j -> forall v,ws[k:=v] = ws) /\
-  (forall i j (bs:list (branch cps)), cpsbranches_wf i j bs ->
-                                      forall k, k >= j -> forall v,bs[k:=v] = bs) /\
-  (forall i j (cs:list cps), fn_list_wf i j cs -> forall k, k >= j -> forall v, cs[k:=v] = cs).
-Proof.
-  apply my_wf_ind ; intros ; simpl ; auto ; 
-  repeat 
-  match goal with
-    | [ H : forall k, k >= ?j -> _, H1 : ?k >= ?j |- _ ] => rewrite (H _ H1) ; auto
-    | _ => idtac
-  end.
-  fold ksubst_branches. rewrite H0 ; auto.
-  repeat if_split.
-  rewrite (H (1+k)) ; auto ; lia.
-  rewrite (H (1+k)) ; auto ; lia.
-  fold ksubst_vals. rewrite H ; auto.
-  fold ksubst_fn_list. rewrite H ; auto.
-  rewrite H ; auto. lia.
-Qed.
-
-Definition ksubst_closed_cps := proj1 ksubst_closed.
-Definition ksubst_closed_val := proj1 (proj2 ksubst_closed).
-Definition ksubst_closed_vals := proj1 (proj2 (proj2 ksubst_closed)).
-Definition ksubst_closed_branches := proj1 (proj2 (proj2 (proj2 ksubst_closed))).
-Definition ksubst_closed_fn_list := proj2 (proj2 (proj2 (proj2 ksubst_closed))).
-
-(** Eliminate a user substitution when the index we are substituting for is
-    out of range. *)
-Lemma usubst_closed :
-  (forall i j (e:cps), cps_wf i j e ->
-       forall k, k >= i -> forall v, e{k:=v} = e) /\
-  (forall i j (w:val_c), val_wf i j w ->
-       forall k, k >= i -> forall v, w{k:=v} = w) /\
-  (forall i j (ws:list val_c), vals_wf i j ws ->
-       forall k, k >= i -> forall v, ws{k:=v} = ws) /\
-  (forall i j (bs:list (branch cps)), cpsbranches_wf i j bs ->
-       forall k, k >= i -> forall v,bs{k:=v} = bs) /\
-  (forall i j (cs:list cps), fn_list_wf i j cs ->
-       forall k, k >= i -> forall v,cs{k:=v} = cs).
-Proof.
- apply my_wf_ind ; intros ; simpl ; auto ; 
-  repeat 
-  match goal with
-    | [ H : forall k, k >= ?j -> _, H1 : ?k >= ?j |- _ ] =>
-                rewrite (H _ H1) ; auto
-    | _ => idtac
-  end.
- - fold usubst_branches. rewrite H0 ; auto.
- - repeat if_split.
- - rewrite (H (1+k)) ; auto ; lia.
- - fold usubst_vals ; rewrite H ; auto.
- - fold usubst_fn_list. rewrite H ; auto.
- - apply f_equal2; try reflexivity.
-   + apply f_equal2; try reflexivity.
-     * rewrite H; auto. admit.
- - rewrite H. auto. reflexivity.
-   *
-rewrite H ; auto. lia.
-  rewrite H ; auto ; lia.
-Qed.
-Definition usubst_closed_val := proj1 (proj2 usubst_closed).
-
-(** We can eliminate substitution for a continuation variable in a CPS'd term. *)
-Lemma cps_cvt_ksubst :
-  forall i e,
-    exp_wf i e ->
-    forall k v, 
-      (cps_cvt e)[k := v] = cps_cvt e.
-Proof.
-  intros. rewrite (ksubst_closed_val _ _ _ (cps_kvar_closed _ _ H)) ; auto.
-  lia.
-Qed.
-Hint Rewrite cps_cvt_ksubst.
-
-(** Eliminating user shifts when out of range. *)
-Lemma ushift_closed' :
-  (forall i j e, cps_wf i j e -> forall k, ushift_cps k i e = e) /\
-  (forall i j v, val_wf i j v -> forall k, ushift_val k i v = v) /\
-  (forall i j vs, vals_wf i j vs -> forall k, ushift_vals k i vs = vs) /\
-  (forall i j bs, cpsbranches_wf i j bs -> forall k, ushift_branches k i bs = bs) /\
-  (forall i j cs, fn_list_wf i j cs -> forall k, ushift_fn_list k i cs = cs).
-Proof.
-  apply my_wf_ind ; simpl ; intros ;
-  fold ushift_branches ; fold ushift_vals ; fold ushift_fn_list ; try congruence.
-  if_split. rewrite H ; rewrite H0 ; auto.
-Qed.
-
-(** Eliminating continuation shifts when out of range. *)
-Lemma kshift_closed' :
-  (forall i j e, cps_wf i j e -> forall k, kshift_cps k j e = e) /\
-  (forall i j v, val_wf i j v -> forall k, kshift_val k j v = v) /\
-  (forall i j vs, vals_wf i j vs -> forall k, kshift_vals k j vs = vs) /\
-  (forall i j bs, cpsbranches_wf i j bs -> forall k, kshift_branches k j bs = bs) /\
-  (forall i j cs, fn_list_wf i j cs -> forall k, kshift_fn_list k j cs = cs).
-Proof.
-  apply my_wf_ind ; simpl ; intros ;
-  fold kshift_branches; fold kshift_vals ; fold kshift_fn_list ; try congruence.
-  if_split. rewrite H ; rewrite H0 ; auto.
-Qed.
-
-Definition kshift_closed_cps := proj1 kshift_closed'.
-Definition kshift_closed_val' := proj1 (proj2 kshift_closed').
-Definition kshift_closed_vals := proj1 (proj2 (proj2 kshift_closed')).
-Definition kshift_closed_branches := proj1 (proj2 (proj2 (proj2 kshift_closed'))).
-Definition kshift_closed_fn_list := proj2 (proj2 (proj2 (proj2 kshift_closed'))).
-
-(** Eliminating user shifts on closed values. *)
-Lemma ushift_closed_val :
-  forall v, val_wf 0 0 v -> forall k l, ushift_val k l v = v.
-Proof.
-  intros.
-  assert (val_wf l 0 v). generalize (val_weaken _ _ _ H l 0). simpl.
-  replace (l + 0) with l ; try lia. auto.
-  eapply (proj1 (proj2 ushift_closed')) ; eauto.
-Qed.
-
-(** Eliminating continuation shifts on closed values. *)
-Lemma kshift_closed_val :
-  forall v, val_wf 0 0 v -> forall k l, kshift_val k l v = v.
-Proof.
-  intros.
-  assert (val_wf 0 l v). generalize (val_weaken _ _ _ H 0 l). simpl.
-  replace (l + 0) with l ; auto ; lia.
-  eapply kshift_closed_val' ; eauto.
-Qed.  
-
-(** A preservation theorem for substitution of a closed value for a
-    user variable. *)
-Lemma usubst_preserves_wf' :
-  (forall i' j e, cps_wf i' j e ->
-                  forall i, i' = 1+i -> 
-                            forall v, val_wf 0 0 v -> forall k, k <= i -> cps_wf i j (e{k := v})) /\
-  (forall i' j w, val_wf i' j w ->
-                  forall i, i' = 1+i -> 
-                            forall v, val_wf 0 0 v -> forall k, k <= i -> val_wf i j (w{k := v})) /\
-  (forall i' j ws, vals_wf i' j ws ->
-                  forall i, i' = 1+i -> 
-                            forall v, val_wf 0 0 v -> forall k, k <= i -> vals_wf i j (ws{k := v})) /\
-  (forall i' j bs, cpsbranches_wf i' j bs ->
-                   forall i, i' = 1+i ->
-                             forall v, val_wf 0 0 v -> forall k, k <= i -> cpsbranches_wf i j (bs{k:=v})) /\
-  (forall i' j cs, fn_list_wf i' j cs ->
-                   forall i, i' = 1+i ->
-                             forall v, val_wf 0 0 v -> forall k, k <= i -> fn_list_wf i j (cs{k:=v})).
-Proof.
-  apply my_wf_ind ; simpl ; intros ; subst ; repeat
-  match goal with
-    | [ H : forall i, 1+?j = 1+i -> _ |- _ ] => specialize (H _ eq_refl)
-    | _ => auto
-  end.
-  repeat if_split ; try (constructor ; auto ; lia). rewrite ushift_closed_val ; auto.
-  specialize (H _ H1). constructor. apply H. lia.
-  constructor ; auto. specialize (H (n + i0)). replace (n + (1 + i0)) with (1 + (n + i0)) in H ;
-    [idtac | lia]. specialize (H eq_refl _ H2). apply (H (n+k)). lia.
-  constructor. apply (H (2 + i0)) ; auto ; try lia.
-  apply H0 ; auto.
-Qed.
-
-Definition usubst_preserves_wf_cps := proj1 usubst_preserves_wf'.
-Definition usubst_preserves_wf_val := proj1 (proj2 usubst_preserves_wf').
-
-(** A preservation theorem for substitution of a closed value for a
-    continuation variable. *)
-Lemma ksubst_preserves_wf' :
-  (forall i j' e, cps_wf i j' e ->
-                  forall j, j' = 1+j -> 
-                            forall v, val_wf 0 0 v -> forall k, k <= j -> cps_wf i j (e[k := v])) /\
-  (forall i j' w, val_wf i j' w ->
-                  forall j, j' = 1+j -> 
-                            forall v, val_wf 0 0 v -> forall k, k <= j -> val_wf i j (w[k := v])) /\
-  (forall i j' ws, vals_wf i j' ws ->
-                  forall j, j' = 1+j -> 
-                            forall v, val_wf 0 0 v -> forall k, k <= j -> vals_wf i j (ws[k := v])) /\
-  (forall i j' bs, cpsbranches_wf i j' bs ->
-                   forall j, j' = 1+j ->
-                             forall v, val_wf 0 0 v -> forall k, k <= j -> cpsbranches_wf i j (bs[k:=v])) /\
-  (forall i j' cs, fn_list_wf i j' cs ->
-                   forall j, j' = 1+j ->
-                             forall v, val_wf 0 0 v -> forall k, k <= j -> fn_list_wf i j (cs[k:=v])).
-Proof.
-  apply my_wf_ind ; simpl ; intros ; subst ; repeat
-  match goal with
-    | [ H : forall i, 1+?j = 1+i -> _ |- _ ] => specialize (H _ eq_refl)
-    | _ => auto
-  end.
-  repeat if_split ; try (constructor ; auto ; lia). rewrite kshift_closed_val ; auto.
-  constructor. apply H ; auto ; lia.
-  constructor ; apply H ; auto ; lia.
-  constructor ; [apply H ; auto ; lia | apply H0 ; auto].
-Qed.
-
-Definition ksubst_preserves_wf_cps := proj1 ksubst_preserves_wf'.
-Definition ksubst_preserves_wf_branches := proj1 (proj2 (proj2 (proj2 ksubst_preserves_wf'))).
-
-(** Substitution preservation specialized to a 0 index on an CPS expression. *)
-Lemma usubst_preserves_wf :
-  forall i j e, cps_wf (1+i) j e -> forall v, val_wf 0 0 v -> cps_wf i j (e{0:=v}).
-Proof.
-  intros. eapply usubst_preserves_wf_cps ; eauto. lia.
-Qed.
-
-(** Substitution preservation specialized to a 0 index on an CPS expression. *)
-Lemma ksubst_preserves_wf :
-  forall i j e, cps_wf i (1+j) e -> forall v, val_wf 0 0 v -> cps_wf i j (e[0:=v]).
-Proof.
-  intros. eapply ksubst_preserves_wf_cps ; eauto. lia.
-Qed.
-
-Lemma find_cps_branch_wf :
-  forall i j bs, cpsbranches_wf i j bs ->
-                 forall d n c, find_branch d n bs = Some c ->
-                               cps_wf (n+i) j c.
-Proof.
-  induction bs ; simpl ; intros ; try discriminate.
-  inversion H ; subst ; clear H. simpl in H0.
-  destruct (N.eq_dec d d0) ; subst.
-  destruct (N.eq_dec n0 n) ; subst ; try discriminate.
-  injection H0 ; intros ; subst ; auto.
-  eapply IHbs ; eauto.
-Qed.
-
-Lemma usubst_list_preserves_wf :
-  forall vs, vals_wf 0 0 vs ->
-             forall c, cps_wf (N.of_nat (length vs)) 0 c ->
-                       cps_wf 0 0 (usubst_list c vs).
-Proof.
-  induction vs ; simpl ; intros ; auto.
-  inversion H ; subst ; clear H.
-  apply (IHvs H6 (usubst_cps a 0 c)).
-  eapply usubst_preserves_wf ; eauto.
-  replace (1 + N.of_nat (length vs)) with (N.of_nat (S (length vs))) ;
-    auto ; lia.
-Qed.
-
-Lemma nth_opt_cps_wf :
-  forall i j cs, fn_list_wf i j cs -> forall n c, nthopt n cs = Some c -> cps_wf (2+i) (1+j) c.
-Proof.
-  induction cs ; simpl ; intros. destruct n ; try discriminate.
-  inversion H ; subst ; clear H. destruct n ; simpl in *.
-  injection H0 ; intros ; subst ; auto.
-  apply (IHcs H6 _ _ H0).
-Qed.
-
-(** Evaluation of CPS terms preserves closedness. *)
-Lemma cps_eval_preserves_wf :
-  forall e v, eval_c e v -> cps_wf 0 0 e -> val_wf 0 0 v.
-Proof.
-  induction 1 ; intros. inversion H ; subst ; auto.
-  inversion H0 ; clear H0 ; subst. inversion H5 ; clear H5 ; subst.
-  apply IHeval_c. apply ksubst_preserves_wf ; auto.
-  inversion H0 ; clear H0 ; subst. inversion H6 ; clear H6 ; subst.
-  apply IHeval_c.
-  apply usubst_preserves_wf ; auto.
-  apply ksubst_preserves_wf ; auto.
-  inversion H1 ; subst ; clear H1.
-  apply IHeval_c.
-  generalize (find_cps_branch_wf _ _ _ H7 _ _ _ H).
-  rewrite N.add_0_r. inversion H6 ; subst ; clear H6 ; intros.
-  apply usubst_list_preserves_wf ; auto.
-  inversion H1 ; subst. clear H1. inversion H6 ; clear H6 ; subst.
-  specialize (nth_opt_cps_wf _ _ _ H4 _ _ H). intros.
-  apply IHeval_c ; clear IHeval_c. constructor ; auto.
-  unfold substitute in *. simpl in *. intros. constructor.
-  apply (usubst_preserves_wf_cps 2 1 c H1 1 eq_refl).
-  constructor ; auto. lia.
-Qed.
-
-(** Getting rid of redundant shifts.  (Duplicate?) *)
-Lemma wf_kshift_zero :
-  (forall i j e, cps_wf i j e -> forall k l, j <= l -> (kshift_cps k l e) = e) /\
-  (forall i j v, val_wf i j v -> forall k l, j <= l -> (kshift_val k l v) = v) /\
-  (forall i j vs, vals_wf i j vs -> forall k l, j <= l -> (kshift_vals k l vs) = vs) /\
-  (forall i j bs, cpsbranches_wf i j bs -> forall k l, j <= l -> (kshift_branches k l bs) = bs)/\
-  (forall i j cs, fn_list_wf i j cs -> forall k l, j <= l -> (kshift_fn_list k l cs) = cs).
-Proof.
-  apply my_wf_ind ; intros ; simpl ; subst ; auto ;
-  try (rewrite H ; auto ; try lia ; rewrite H0 ; auto ; rewrite H1 ; auto).
-  if_split.
-Qed.
-
-Definition wf_kshift_zero_val := proj1 (proj2 wf_kshift_zero).
-
-Lemma is_valueb_shift' :
-  (forall e i j, is_valueb (shift i j e) = is_valueb e) /\ 
-  (forall es i j, are_valuesb (shifts i j es) = are_valuesb es) /\
-  (forall (bs:list (branch exp)), True).
-Proof.
-  apply my_exp_ind ; simpl ; intros ; auto. rewrite H. rewrite H0. auto.
-Qed.
-
-Definition is_valueb_shift := proj1 is_valueb_shift'.
-Definition are_valuesb_shift := proj1 (proj2 is_valueb_shift').
-
-Lemma is_value_shift' :
-  (forall e i j, is_value (shift i j e) <-> is_value e) /\ 
-  (forall es i j, are_values (shifts i j es) <-> are_values es) /\
-  (forall (bs:list (branch exp)), True).
-Proof.
-  apply my_exp_ind ; simpl ; intros ; split ; intro ; auto ;
-  try (inversion H1 ; fail). inversion H0 ; subst. constructor.
-  rewrite <- H ; eauto. inversion H0 ; subst. constructor.
-  rewrite H ; eauto. inversion H0. inversion H0.
-  inversion H1. subst. constructor. rewrite <- H ; eauto.
-  rewrite <- H0 ; eauto. inversion H1 ; subst ; constructor. rewrite H ; eauto.
-  rewrite H0 ; eauto.
-Qed.
-
-Definition is_value_shift := proj1 is_value_shift'.
-Definition are_values_shift := proj1 (proj2 is_value_shift').
-
-Lemma length_shift :
-  forall es i j, length (shifts i j es) = length es.
-Proof.
-  intros ; unfold shifts, shifts'. apply map_length.
-Qed.
-
-Lemma ushift_list_to_indices :
-  forall es i j, ushift_vals i j (list_to_indices es) = list_to_indices (shifts i j es).
-Proof.
-  induction es ; simpl ; intros ; auto. rewrite length_shift. congruence.
-Qed.
-
-(** User variable shifts commute with CPS conversion. *)
-Lemma ushift_cps_cvt' :
-  (forall e, (forall i j,ushift_val i j (cps_cvt e) = cps_cvt (shift i j e)) /\
-                 (is_value e -> forall i j, (ushift_val i j (cps_cvt_val e) =
-                                             cps_cvt_val (shift i j e))))
-  /\
-  (forall es, (forall i j c,
-                 ushift_cps i j (cps_cvts es c) = cps_cvts (shifts i j es) (ushift_cps i j c)) /\
-              (are_values es -> forall i j, (ushift_vals i j (cps_cvt_vals es) =
-                                             cps_cvt_vals (shifts i j es))) /\
-              (forall i j,
-                 ushift_fn_list i j (cps_cvt_fn_list es) = cps_cvt_fn_list (shifts i (2 + j) es)))
-  /\
-  (forall bs i j,
-     ushift_branches i j (cps_cvt_branches bs) = cps_cvt_branches (shift_branches i j bs)).
-Proof.
-  apply my_exp_ind ; simpl ; intros ; auto.
-  split ; intros.
-  rewrite (proj1 H). auto.
-  rewrite (proj1 H). auto.
-  split ; intros.
-  rewrite (proj1 H) ; rewrite (proj1 H0) ; auto.
-  inversion H1.
-  fold are_valuesb. fold cps_cvt_val. fold cps_cvt_vals.
-  split ; intros.
-  generalize (proj1 (are_valuesb_corr es)). destruct H. intros.
-  rewrite (are_valuesb_shift). destruct (are_valuesb es) ; simpl ; auto.
-  rewrite (proj1 H0) ; auto. rewrite H ; auto. simpl. rewrite length_shift.
-  rewrite ushift_list_to_indices. auto. inversion H0 ; subst.
-  rewrite (proj1 (proj2 H) H2). auto.
-  intros. split ; [ intros | intro H1 ; inversion H].
-  rewrite (proj1 H). fold ushift_branches. fold shift_branches.
-  rewrite H0. auto.
-  inversion H1.
-  split ; intros.
-  rewrite (proj1 H) ; rewrite (proj1 H0) ; auto.
-  inversion H1.
-  split ; intros.
-  fold ushift_fn_list cps_cvt_fn_list shifts.
-  rewrite (proj2 (proj2 H)). auto.
-  rewrite (proj2 (proj2 H)). auto.
-  split ; intros.
-  rewrite (proj1 H) ; auto. inversion H0.
-  split ; intros.
-  rewrite (proj1 H) ; rewrite (proj1 H0) ; auto.
-  split ; intros.
-  inversion H1 ; subst. clear H1. rewrite (proj2 H H4).
-  rewrite (proj1 (proj2 H0) H5). auto. 
-  rewrite (proj1 H). rewrite (proj2 (proj2 H0)). auto.
-  rewrite (proj1 H) ; auto. rewrite H0 ; auto.
-Qed.
-
-Lemma ushift_cps_cvt e i j : ushift_val i j (cps_cvt e) = cps_cvt (shift i j e).
-  apply (proj1 (proj1 ushift_cps_cvt' e) i j).
-Qed.
-
-Lemma ushift_cps_cvt_val e i j :
-  is_value e -> ushift_val i j (cps_cvt_val e) = cps_cvt_val (shift i j e).
-Proof.
-  intro H. apply (proj2 (proj1 ushift_cps_cvt' e) H i j).
-Qed.
-
-Lemma ushift_cps_cvts es i j c :
-  ushift_cps i j (cps_cvts es c) = cps_cvts (shifts i j es) (ushift_cps i j c).
-Proof.
-  apply (proj1 (proj1 (proj2 ushift_cps_cvt') es) i j c).
-Qed.
-
-Lemma ushift_cps_cvt_vals es i j :
-  are_values es -> ushift_vals i j (cps_cvt_vals es) = cps_cvt_vals (shifts i j es).
-Proof.
-  intro H. apply (proj1 (proj2 (proj1 (proj2 ushift_cps_cvt') es)) H i j).
-Qed.
-
-Lemma ushift_cps_cvt_fn_list es i j :
-  ushift_fn_list i j (cps_cvt_fn_list es) = cps_cvt_fn_list (shifts i (2 + j) es).
-Proof.
-  apply (proj2 (proj2 ((proj1 (proj2 ushift_cps_cvt') es)))).
-Qed.
-Lemma ushift_cps_cvt_branches bs i j :
-  ushift_branches i j (cps_cvt_branches bs) = cps_cvt_branches (shift_branches i j bs).
-Proof.
-  apply (proj2 (proj2 ushift_cps_cvt')).
-Qed.
-
-Lemma is_valueb_subst' :
-  forall v, is_value v ->
-            (forall e i, is_valueb (subst v i e) = is_valueb e) /\
-            (forall es i, are_valuesb (substs v i es) = are_valuesb es) /\
-            (forall bs : list (branch exp), True).
-Proof.
-  intros v H.
-  apply my_exp_ind ; simpl ; intros ; auto. repeat if_split.
-  rewrite (is_valueb_shift). rewrite (is_valueb_corr v) ; auto.
-  rewrite H0. rewrite H1. auto.
-Qed.
-
-Lemma is_valueb_subst v e i :
-  is_value v -> is_valueb (subst v i e) = is_valueb e.
-  intro H. apply (proj1 (is_valueb_subst' v H) e i).
-Qed.
-
-Lemma are_valuesb_subst v es i :
-  is_value v -> are_valuesb (substs v i es) = are_valuesb es.
-  intro H. apply (proj1 (proj2 (is_valueb_subst' v H)) es i).
-Qed.
-  
-Lemma length_substs :
-  forall es v j, length (substs v j es) = length es.
-Proof.
-  unfold substs, substs'. intros. rewrite map_length. auto.
-Qed.
-
-Lemma list_to_indices_substs :
-  forall es v j, list_to_indices (substs v j es) = list_to_indices es.
-Proof.
-  induction es ; simpl ; intros ; auto. rewrite length_substs. congruence.
-Qed.
-
-Lemma usubst_list_to_indices :
-  forall es v j, usubst_vals v j (list_to_indices es) = list_to_indices es.
-Proof.
-  induction es ; simpl ; intros ; congruence.
-Qed.
-
-Lemma wf_list_to_indices :
-  forall es, vals_wf 0 (1 + (N.of_nat (length es))) (list_to_indices es).
-Proof.
-  induction es ; simpl ; repeat constructor ; try lia ; auto.
-  generalize (vals_weaken _ _ _ IHes 0 1).
-  replace (1 + (1 + N.of_nat (length es))) with (1 + N.of_nat (S (length es))) ;
-    auto ; try lia.
-Qed.
-
-(** CPS conversion commutes with substitution for user variables. *)
-Lemma cps_cvt_comm_usubst':
-  forall v, is_value v -> exp_wf 0 v ->
-  (forall i e, exp_wf i e ->
-    (forall j, j < i ->       
-      (usubst_val (cps_cvt_val v) j (cps_cvt e) = cps_cvt (subst v j e))) /\
-    (forall j, j < i -> 
-      (is_valueb e = true ->        
-       (usubst_val (cps_cvt_val v) j (cps_cvt_val e) =
-        cps_cvt_val (subst v j e))))) /\
-  (forall i es, exps_wf i es ->
-     (forall j k c,
-        j < i -> cps_wf 0 k c -> 
-        usubst_cps (cps_cvt_val v) j (cps_cvts es c) =
-        cps_cvts (substs v j es) (usubst_cps (cps_cvt_val v) j c)) /\
-     (are_valuesb es = true -> 
-      forall j, j < i ->
-                usubst_vals (cps_cvt_val v) j (cps_cvt_vals es) =
-                cps_cvt_vals (substs v j es)) /\
-     (forall j i', i = 2 + i' ->  j < i' ->
-                   usubst_fn_list (cps_cvt_val v) j (cps_cvt_fn_list es) =
-                   cps_cvt_fn_list (substs v (2+j) es))) /\
-  (forall i bs, branches_wf i bs ->
-     forall j, j < i -> 
-               usubst_branches (cps_cvt_val v) j (cps_cvt_branches bs) =
-               cps_cvt_branches (subst_branches v j bs)).
-Proof.
-  intros v H1 H2.
-  apply my_exp_wf_ind ; simpl ; intros ; auto ; try split ; intros ; 
-  repeat match goal with [ H : _ /\ _ |- _ ] => destruct H | _ => idtac end ;
-  try discriminate.
-  repeat if_split.
-  rewrite (ushift_cps_cvt_val v) ; auto. rewrite cps_val ; auto.
-  apply is_value_shift ; auto.
-  repeat if_split. apply ushift_cps_cvt_val ; auto.
-  assert (H4: 1+j < 1+i) ; [lia | rewrite (H _ H4); auto].
-  assert (H5: 1+j < 1+i) ; [lia | rewrite (H _ H5); auto].
-  rewrite H ; auto ; rewrite H0 ; auto. 
-  rewrite (are_valuesb_subst) ; auto. fold are_valuesb.
-  remember (are_valuesb es) as b. destruct b. simpl.
-  fold cps_cvt_val cps_cvt_vals substs.
-  rewrite H3 ; auto.
-  rewrite list_to_indices_substs ; rewrite length_substs. simpl.
-  rewrite (H _ (1+ (N.of_nat (length es)))) ; eauto. simpl. 
-  rewrite usubst_list_to_indices ; auto.
-  repeat constructor ; try lia. apply wf_list_to_indices.
-  rewrite (H4 H3) ; auto.
-  rewrite H ; auto. fold cps_cvt_branches usubst_branches subst_branches.
-  rewrite H0 ; auto.
-  rewrite H0 ; auto. rewrite H ; auto. lia.
-  fold usubst_fn_list cps_cvt_fn_list substs. rewrite (H4 j i); auto. 
-  fold usubst_fn_list cps_cvt_fn_list substs'. rewrite (H5 j i) ; auto. 
-  rewrite H ; auto.
-  erewrite H0 ; eauto. rewrite H ; auto.
-  split.
-  remember (is_valueb e) as b1.
-  remember (are_valuesb es) as b2.
-  destruct b1 ; destruct b2 ; intros ; try discriminate. 
-  rewrite H5 ; auto. rewrite H3 ; auto. 
-  intros. subst. rewrite (H4 _ _ eq_refl); auto. rewrite H ; auto. lia.
-  rewrite H ; auto ; try lia. rewrite H0 ; auto.
-Qed.
-
-Lemma cps_cvt_comm_subst :
-  forall v i e j, is_value v -> exp_wf 0 v -> exp_wf i e -> j < i ->
-       usubst_val (cps_cvt_val v) j (cps_cvt e) = cps_cvt (subst v j e).
-Proof.
-  intros. apply (proj1 (proj1 (cps_cvt_comm_usubst' v H H0) i e H1) j H2).
-Qed.
-
-Lemma cps_cvt_val_comm_subst :
-  forall v i e j, is_value v -> exp_wf 0 v -> exp_wf i e -> j < i ->
-    is_valueb e = true -> 
-    usubst_val (cps_cvt_val v) j (cps_cvt_val e) = cps_cvt_val (subst v j e).
-Proof.
-  intros. apply (proj2 (proj1 (cps_cvt_comm_usubst' v H H0) i e H1) j H2 H3).
-Qed.
-
-Lemma cps_cvts_comm_subst :
-  forall v i es j k c, is_value v -> exp_wf 0 v -> exps_wf i es -> j < i ->
-    cps_wf 0 k c ->
-    usubst_cps (cps_cvt_val v) j (cps_cvts es c) =
-    cps_cvts (substs v j es) (usubst_cps (cps_cvt_val v) j c).
-Proof.
-  intros. apply (proj1 (proj1 (proj2 (cps_cvt_comm_usubst' v H H0)) i es H1) j k c H2 H3).
-Qed.
-
-Lemma cps_cvt_vals_comm_subst :
-  forall v i es j, is_value v -> exp_wf 0 v -> exps_wf i es ->
-      are_valuesb es = true -> j < i -> 
-      usubst_vals (cps_cvt_val v) j (cps_cvt_vals es) =
-      cps_cvt_vals (substs v j es).
-Proof.
-  intros.
-  apply (proj1 (proj2 (proj1 (proj2 (cps_cvt_comm_usubst' v H H0)) i es H1)) H2 j H3).
-Qed.
-
-Lemma cps_cvt_branches_comm_subst :
-  forall v i bs j, is_value v -> exp_wf 0 v -> branches_wf i bs -> j < i -> 
-                   usubst_branches (cps_cvt_val v) j (cps_cvt_branches bs) =
-                   cps_cvt_branches (subst_branches v j bs).
-Proof.
-  intros. apply (proj2 (proj2 (cps_cvt_comm_usubst' v H H0)) i bs H1 j H2).
-Qed.
-
-Lemma cps_cvt_fn_list_comm_subst :
-  forall v i es j, is_value v -> exp_wf 0 v -> exps_wf (2 + i) es -> j < i ->
-                   usubst_fn_list (cps_cvt_val v) j (cps_cvt_fn_list es) =
-                   cps_cvt_fn_list (substs v (2+j) es).
-Proof.
-  intros. 
-  apply (proj2 (proj2 (proj1 (proj2 (cps_cvt_comm_usubst' v H H0)) _ es H1)) j i eq_refl H2).
-Qed.
-
-Lemma cps_cvt_comm_usub_list :
-  forall vs, are_values vs -> exps_wf 0 vs ->
-             forall e k, exp_wf (N.of_nat (length vs)) e -> val_wf 0 0 k -> 
-                         usubst_list (Ret_c (cps_cvt e) k) (cps_cvt_vals vs) =
-                         (Ret_c (cps_cvt (subst_list e vs)) k).
-Proof.
-  induction vs ; simpl ; intros. auto. inversion H. inversion H0. subst ; clear H H0.
-  erewrite cps_cvt_comm_subst ; eauto ; try lia.
-  erewrite usubst_closed_val ; eauto ; try lia.
-  apply IHvs ; eauto. apply subst_preserves_exp_wf ; auto.
-  replace (1 + N.of_nat (length vs)) with (N.of_nat (S (length vs))) ; auto ; lia.
-Qed.
-
-Lemma evals_length :
-  forall es vs, evals es vs -> length es = length vs.
-Proof.
-  induction es ; intros vs H ; inversion H ; intros ; subst ; auto.
-  simpl. rewrite (IHes vs0) ; auto.
-Qed.
-
-Lemma evals_list_to_indices :
-  forall es vs, evals es vs -> list_to_indices es = list_to_indices vs.
-Proof.
-  induction es. intros. inversion H ; subst. auto. intros.
-  inversion H ; intros ; subst. simpl. erewrite evals_length ; eauto.
-  erewrite IHes ; eauto.
-Qed.    
-
-Lemma eval_is_valueb_eq' : 
-  (forall e v,
-     eval e v ->
-     true = is_valueb e -> e = v) /\
-  (forall es vs, 
-        evals es vs -> 
-        true = are_valuesb es -> es = vs).
-Proof.
-  apply my_eval_ind ; simpl ; intros ; auto ; try discriminate.
-  rewrite H ; auto.
-  destruct (is_valueb e) ; destruct (are_valuesb es) ; try discriminate.
-  rewrite (H eq_refl) ; rewrite (H0 eq_refl) ; auto.
-Qed.
-
-Definition eval_is_valueb_eq := proj1 eval_is_valueb_eq'.
-Definition evals_are_valuesb_eq := proj2 eval_is_valueb_eq'.
-
-Lemma ksubst_gt_indices :
-  forall k es i, i >= N.of_nat (length es) ->
-                 ksubst_vals k i (list_to_indices es) = list_to_indices es.
-Proof.
-  induction es ; simpl ; intros ; auto. if_split. rewrite IHes ; auto. lia.
-Qed.
-
-Lemma ksubst_cps_cvts' : 
-  forall d k, val_wf 0 0 k -> 
-    forall es2 es1, exps_wf 0 es2 -> 
-      (cps_cvts es2 (Ret_c (KVar_c (N.of_nat (length (es1 ++ es2))))
-                           (Con_c d (list_to_indices (es1 ++ es2)))))[N.of_nat(length es1) := k] =
-      cps_cvts es2 (Ret_c k (Con_c d (list_to_indices (es1 ++ es2)))).
-Proof.
-  induction es2 ; simpl ; intros.
-  repeat if_split ; try rewrite <- app_nil_end in * ; try lia.
-  erewrite kshift_closed_val ; eauto.
-  rewrite ksubst_gt_indices ; auto ; lia.
-  inversion H0 ; clear H0 ; subst.
-  erewrite ksubst_closed_val. Focus 2.
-  eapply cps_kvar_closed. eauto. Focus 2. lia. repeat apply f_equal.
-  specialize (IHes2 (es1 ++ [a]) H5).
-  repeat rewrite app_length in *. simpl in *.
-  repeat rewrite <- app_assoc in IHes2. simpl in *.
-  replace (N.of_nat (length es1 + 1)) with (1 + N.of_nat (length es1)) in IHes2 ; try lia. 
-  replace (N.of_nat (length es1 + 1 + length es2)) with (N.of_nat (length es1 + S (length es2)))
-  in IHes2; try lia. auto.
-Qed.
-
-Lemma ksubst_cps_cvts :
-  forall d k es,
-    val_wf 0 0 k ->
-    exps_wf 0 es ->
-      (cps_cvts es (Ret_c (KVar_c (N.of_nat (length es)))
-                           (Con_c d (list_to_indices es))))[0 := k] =
-      cps_cvts es (Ret_c k (Con_c d (list_to_indices es))).
-Proof.
-  intros. generalize (ksubst_cps_cvts' d k H es nil H0). simpl. auto.
-Qed.
-
-Lemma ksubst_vals_append :
-  forall v k (vs1 vs2:list val_c),
-    (vs1 ++ vs2)[k:=v] = (vs1[k:=v]) ++ (vs2[k:=v]).
-  induction vs1 ; simpl ; intros ; auto. rewrite IHvs1. auto.
-Qed.
-
-Lemma ksubst_cps_cvts2' :
-  forall es2 es1,
-    exps_wf 0 es2 ->
-    forall v k,
-      (cps_cvts es2 k) [N.of_nat(length es1) := (cps_cvt_val v)] = 
-      (cps_cvts es2 (k [N.of_nat(length (es1 ++ es2)) := (cps_cvt_val v)])).
-Proof.
-  induction es2 ; simpl ; intros ; auto.
-  rewrite <- app_nil_end ; auto.
-  inversion H ; clear H ; subst.
-  erewrite cps_cvt_ksubst ; eauto. repeat apply f_equal.
-  specialize (IHes2 (es1 ++ [a]) H4).
-  repeat rewrite app_length in *. simpl in *.
-  replace (N.of_nat (length es1 + 1)) with (1 + N.of_nat (length es1)) in IHes2 ; try lia.
-  rewrite IHes2.
-  replace (N.of_nat (length es1 + 1 + length es2)) with (N.of_nat (length es1 + S (length es2))) ;
-    auto ; try lia.
-Qed.
-
-Lemma ksubst_cps_cvts2 :
-  forall es v k, exps_wf 0 es ->
-                 (cps_cvts es k) [0 := cps_cvt_val v] =
-                 cps_cvts es (k [N.of_nat (length es) := cps_cvt_val v]).
-Proof.
-  intros.
-  apply (ksubst_cps_cvts2' es nil H v k).
-Qed.                 
-
-Fixpoint cps_cvt_vals' (es:list exp) (k:cps) : cps :=
-  match es with
-    | nil => k
-    | e :: es => cps_cvt_vals' es (k[N.of_nat(length es):=cps_cvt_val e])
-  end.
-
-Lemma vals_wf_append :
-  forall i j vs1 vs2,
-    vals_wf i j (vs1 ++ vs2) <-> (vals_wf i j vs1 /\ vals_wf i j vs2).
-Proof.
-  induction vs1 ; simpl ; intros ; split ; intro. split. constructor. auto.
-  destruct H ; auto. inversion H ; subst ; clear H. split ; auto. 
-  constructor ; auto. specialize (IHvs1 vs2). destruct IHvs1. tauto.
-  specialize (IHvs1 vs2). destruct IHvs1. tauto.
-  destruct H. inversion H. subst. clear H. constructor ; auto.
-  specialize (IHvs1 vs2). destruct IHvs1. auto.
-Qed.
-
-Lemma eval_cps_cvt_vals' :
-  forall d vs,
-    exps_wf 0 vs -> 
-    are_values vs ->
-    forall k ws,
-      val_wf 0 0 k ->
-      vals_wf 0 0 ws ->
-      forall v', 
-        (eval_c (cps_cvt_vals' vs (Ret_c k (Con_c d (ws ++ (list_to_indices vs))))) v' <->
-         eval_c (Ret_c k (Con_c d (ws ++ (cps_cvt_vals vs)))) v').
-Proof.
-  induction vs ; simpl ; intros. tauto.
-  inversion H ; inversion H0 ; subst ; clear H H0. rename a into v.
-  erewrite (ksubst_closed_val 0 0) ; auto ; try lia.
-  fold ksubst_vals. rewrite ksubst_vals_append.
-  erewrite ksubst_closed_vals ; eauto ; try lia.
-  simpl. repeat if_split.
-  erewrite kshift_closed_val ; [idtac | eapply cps_val_kvar_closed ; eauto].
-  rewrite ksubst_gt_indices ; try lia.
-  specialize (app_assoc ws [cps_cvt_val v] (list_to_indices vs)).
-  intros. simpl in H. rewrite H.
-  specialize (IHvs H7 H11 k (ws ++ [cps_cvt_val v]) H1).
-  rewrite IHvs. rewrite <- app_assoc ; simpl ; tauto.
-  rewrite vals_wf_append ; split ; auto. 
-Qed.
-
-Lemma find_branch_cps_cvt :
-  forall d n e bs,
-    find_branch d n bs = Some e ->
-    forall v1 v2,
-      find_branch d n (ksubst_branches v1 0 (ksubst_branches v2 1 (cps_cvt_branches bs))) =
-      Some (ksubst_cps v1 0 (ksubst_cps v2 1 (Ret_c (cps_cvt e) (KVar_c 1)))).
-Proof.
-  induction bs ; simpl ; intros. discriminate. unfold br.
-  destruct a. destruct p. simpl in *. repeat if_split. congruence. discriminate.
-Qed.
-
-Lemma cps_cvt_list_nth :
-  forall n es e, nthopt n es = Some e ->
-    nthopt n (cps_cvt_fn_list es) = Some (Ret_c (cps_cvt e) (KVar_c 0)).
-Proof.
-  induction n ; destruct es ; simpl ; intros ; try discriminate. injection H.
-  intro ; subst ; auto. apply (IHn _ _ H).
-Qed.
-
-(** The key correctness lemma for CPS conversion.  In essence, CPS converting
-    an expression and feeding it closed continuation [k], is the same as 
-    evaluating the expression to a value, then CPS converting the value,
-    and then feeding k to the value. *)
-Lemma cps_cvt_corr :
-  (forall e v,
-     eval e v ->
-     exp_wf 0 e -> 
-     forall k, val_wf 0 0 k ->
-               forall v', 
-                 eval_c (Ret_c (cps_cvt e) k) v' <->
-                 eval_c (Ret_c (cps_cvt v) k) v') /\
-  (forall es vs,
-     evals es vs ->
-     exps_wf 0 es ->
-       forall d k ws,
-         val_wf 0 0 k -> 
-         vals_wf 0 0 ws -> 
-         forall v', 
-           (eval_c (cps_cvts es (Ret_c k (Con_c d (ws ++ (list_to_indices es))))) v' <->
-            eval_c (cps_cvt_vals' vs (Ret_c k (Con_c d (ws ++ (list_to_indices vs))))) v')).
-Proof.
-  Transparent N.add.
-  Transparent N.sub.
-  apply my_eval_ind ; intros ; simpl ; try tauto.
-  (* application case *)
-  inversion H2 ; clear H2 ; subst.
-  specialize (H H7). specialize (H0 H8).
-  generalize (eval_preserves_wf _ _ e H7) (eval_preserves_wf _ _ e0 H8).
-  intros. inversion H2. subst.
-  generalize (subst_preserves_exp_wf 0 e1' H9 _ H4). intro.
-  generalize (eval_preserves_wf _ _ e3 H5). intro.
-  rewrite <- H1 ; auto ; clear H1.
-  rewrite eval_ret. simpl.
-  rewrite (cps_cvt_ksubst _ _ H7).
-  rewrite (cps_cvt_ksubst _ _ H8).
-  rewrite (kshift_closed_val k H3).
-  rewrite H ; simpl ; clear H. Focus 2. repeat constructor ; eauto.
-  rewrite eval_ret. simpl.
-  rewrite eval_ret. simpl.
-  rewrite (cps_cvt_ksubst (1+0)) ; auto.
-  rewrite (kshift_closed_val' 1 1 (cps_cvt e1')) ; auto. Focus 2.
-  eapply (val_weaken 1 0 (cps_cvt e1') _ 0 1). 
-  rewrite (kshift_closed_val' 0 1 (cps_cvt e2)) ; auto. 
-  rewrite (ksubst_closed_val 0 0 (cps_cvt e2)) ; auto ; try lia.
-  rewrite H0 ; simpl ; clear H0.
-  Focus 2. repeat constructor.
-  eapply (val_weaken 1 0 (cps_cvt e1') _ 0 2). simpl.
-  generalize (cps_kvar_closed _ _ H9). simpl. intro.
-  rewrite (wf_kshift_zero_val 0 0 k H3) ; try lia.
-  rewrite (ksubst_closed_val _ _ _ H3) ; auto ; try lia.
-  generalize (eval_yields_value _ _ e0). intro. 
-  rewrite (cps_val _ H).
-  rewrite eval_ret. simpl.
-  repeat rewrite val_kshift_0.
-  generalize (cps_val_kvar_closed 0 _ H4 H). intro.
-  rewrite (ksubst_closed_val _ _ (cps_cvt_val v2) H0 0) ; auto ; try lia.
-  rewrite eval_ret. simpl.
-  repeat rewrite val_kshift_0.
-  repeat rewrite (ksubst_closed_val _ _ _ H3) ; auto ; try lia.
-  rewrite eval_call. simpl.
-  rewrite val_kshift_0. 
-  generalize (cps_kvar_closed _ _ H9). intro.
-  generalize (val_weaken _ _ _ H1 0 1). simpl. intro.
-  repeat rewrite (ksubst_closed_val _ _ _ H1) ; auto ; try lia.
-  rewrite (usubst_closed_val _ _ _ H3) ; auto ; try lia.
-  rewrite (cps_cvt_comm_subst v2 1) ; auto ; try lia.
-  tauto.
-  (* D(e1,....,en) case *)
-  inversion H0 ; clear H0 ; subst. fold are_valuesb.
-  remember (are_valuesb es) as b.
-  generalize (evals_are_valuesb_eq _ _ e). intro.
-  destruct b.
-  (* D(v1,...,vn) case -- already a value *)
-  rewrite Heqb in H0. specialize (H0 eq_refl). subst.
-  rewrite <- Heqb. tauto.
-  (* D(e1,...,en) case -- not already a value *)
-  generalize (proj2 (are_valuesb_corr vs) (evals_yields_values _ _ e)).
-  intro. rewrite H2.
-  repeat rewrite eval_ret.
-  simpl. rewrite val_kshift_0.
-  generalize (ksubst_closed_vals 0 0). unfold ksubstitute. simpl.
-  intros. rewrite H3 ; try lia.
-  Focus 2.
-  apply cps_vals_kvar_closed.
-  apply (evals_preserves_wf _ _ e) ; auto.
-  eapply evals_yields_values ; eauto.
-  rewrite ksubst_cps_cvts ; auto.
-  specialize (H H4 d k nil H1 (nil_c_wf 0 0) v'). simpl in H.
-  rewrite H.
-  assert (are_values vs). apply (proj1 (are_valuesb_corr _)) ; auto.
-  assert (exps_wf 0 vs). eapply (evals_preserves_wf) ; eauto.
-  rewrite (eval_cps_cvt_vals' d vs H6 H5 k nil H1) ; auto. simpl ; tauto.
-  (* Let case *)
-  inversion H1 ; clear H1 ; subst.
-  repeat rewrite eval_ret ; simpl.
-  rewrite (ksubst_closed_val 0 0) ; eauto ; try lia.
-  rewrite H ; eauto.
-  Focus 2. repeat constructor. rewrite (ksubst_closed_val 1 0) ; eauto ; try lia.
-  simpl in *. eapply (val_weaken 1 0 (cps_cvt e2) _ 0 2).
-  rewrite kshift_closed_val ; eauto.
-  rewrite (cps_val v1) ; [idtac | eapply eval_yields_value ; eauto].
-  rewrite eval_ret. simpl. rewrite (ksubst_closed_val 0 0 (cps_cvt_val v1)) ; try lia.
-  Focus 2. apply cps_val_kvar_closed ; eauto. eapply eval_preserves_wf ; eauto.
-  repeat rewrite val_kshift_0.
-  rewrite kshift_closed_val ; eauto. 
-  rewrite eval_ret. simpl.
-  rewrite (ksubst_closed_val 1 0 (cps_cvt e2)) ; try lia.
-  Focus 2. apply (cps_kvar_closed 1) ; auto.
-  rewrite val_kshift_0.
-  rewrite (ksubst_closed_val 1 0 (cps_cvt e2)) ; try lia.
-  Focus 2. apply (cps_kvar_closed 1) ; auto.
-  rewrite (ksubst_closed_val 0 0 k) ; eauto ; try lia.
-  rewrite eval_call. simpl. rewrite (ksubst_closed_val 1 0 (cps_cvt e2)) ; try lia.
-  Focus 2. apply (cps_kvar_closed 1) ; auto.
-  rewrite val_kshift_0. rewrite (usubst_closed_val 0 0 k) ; auto ; try lia.
-  rewrite (cps_cvt_comm_subst v1 1) ; eauto ; try lia.
-  Focus 2. eapply eval_preserves_wf ; eauto.
-  unfold substitute in H0. simpl in H0. apply H0 ; auto.
-  apply subst_preserves_exp_wf ; eauto. eapply eval_preserves_wf ; eauto.
-  (* Match case *)
-  inversion H1 ; subst.
-  assert (is_value (Con_e d vs)). eapply eval_yields_value ; eauto. inversion H3 ; subst.
-  assert (exp_wf 0 (Con_e d vs)). eapply eval_preserves_wf ; eauto. inversion H4 ; subst.
-  rewrite eval_ret. simpl. rewrite (ksubst_closed_val 0 0 (cps_cvt e)) ; eauto ; try lia.
-  assert(cpsbranches_wf 0 1 (ksubst_branches' ksubst_cps k 1 (cps_cvt_branches' cps_cvt bs))).
-  fold ksubst_branches.
-  eapply ksubst_preserves_wf_branches ; eauto ; try lia.
-  apply cps_branches_closed ; auto.
-  rewrite H ; eauto. Focus 2. repeat constructor. eauto.
-  rewrite cps_val ; eauto.
-  rewrite eval_ret. simpl. fold kshift_branches ksubst_branches ksubst_vals cps_cvt_branches.
-  rewrite (kshift_closed_branches 0) ; eauto.
-  rewrite (ksubst_closed_vals 0 0) ; eauto ; try lia.
-  rewrite eval_ret. simpl. fold ksubst_branches kshift_vals cps_cvt_vals.
-  rewrite vals_kshift_0. fold ksubst_branches in H8.
-  generalize (find_branch_cps_cvt _ _ _ _ e1 (Con_c d (cps_cvt_vals vs)) k).
-  assert (length vs = length (cps_cvt_vals vs)). unfold cps_cvt_vals. rewrite map_length. auto.
-  rewrite H9. intro.
-  rewrite eval_match ; eauto.
+  simpl. intros ? Hcl Hisv.  rewrite Hcl.
+  induction Hisv; intros; simpl;
+  unfold cps_cvt; try rewrite Hcl;
+  simpl; auto;[| |];
+  unfold cps_cvt_val; rewrite Hcl; 
+  try(simpl; reflexivity; fail);[].
   simpl.
-  generalize (find_branch_preserves_wf _ _ H7 _ _ _ e1). rewrite N.add_0_r. intro.
-  assert (val_wf (N.of_nat (length vs)) 0 (cps_cvt e')).
-  apply (cps_kvar_closed) ; auto.
-  repeat (rewrite (ksubst_closed_val (N.of_nat (length vs)) 0 (cps_cvt e')) ; eauto ; try lia).
-  rewrite kshift_closed_val ; eauto.
-  rewrite (ksubst_closed_val 0 0 k) ; eauto ; try lia.
-  rewrite cps_cvt_comm_usub_list ; auto. 
-  apply H0 ; auto.
-  apply subst_list_preserves_exp_wf ; auto. rewrite N.add_0_r ; auto.
-  (* Proj case *)
-  inversion H0 ; subst ; clear H0.
-  repeat rewrite eval_ret.
-  simpl. rewrite (kshift_closed_val k) ; eauto. 
-  rewrite (ksubst_closed_val 0 0) ; eauto ; try lia.
-  rewrite H ; auto. Focus 2. repeat constructor. eapply (val_weaken 0 0 k H1 0 1).
-  rewrite val_kshift_0. simpl.
-  rewrite eval_ret. simpl. fold ksubst_fn_list. fold cps_cvt_fn_list.
-  assert (exps_wf 2 es).
-  generalize (eval_preserves_wf _ _ e0 H4). intro. inversion H0 ; subst. auto.
-  assert (fn_list_wf 0 0 (cps_cvt_fn_list es)).
-  apply (cps_fn_list_closed 0 es) ; auto.
-  rewrite (ksubst_closed_fn_list 0 0) ; auto ; try lia.
-  rewrite (kshift_closed_val' 0 1 k) ; [idtac | eapply (val_weaken 0 0 k H1 0 1)].
-  rewrite eval_ret. simpl. fold kshift_fn_list.
-  rewrite (kshift_closed_fn_list _ _ _ H2).
-  rewrite (ksubst_closed_val 0 0 k) ; eauto ; try lia.
-  generalize (cps_cvt_list_nth _ _ _ e1) ; intro.
-  rewrite eval_proj ; eauto.
-  replace (Fix_c (cps_cvt_fn_list es)) with (cps_cvt_val (Fix_e es)) ; auto.
-  replace (Lam_c (Ret_c (cps_cvt e') (KVar_c 0))) with (cps_cvt_val (Lam_e e')) ; auto.
-  rewrite (cps_cvt_val_comm_subst _ 1) ; auto ; try lia. Focus 2.
-  constructor. apply (nthopt_preserves_wf _ _ H0 _ _ e1).
-  rewrite (ksubst_closed_val 1 1) ; try lia. simpl. tauto.
-  rewrite <- (cps_cvt_comm_subst _ 2) ; eauto ; try lia ; simpl.
-  Focus 2. apply (nthopt_preserves_wf _ _ H0 _ _ e1). fold cps_cvt_fn_list.
-  apply (fun H1 H2 H3 => usubst_preserves_wf_val 2 1 (cps_cvt e') H1 1 H2 (Fix_c (cps_cvt_fn_list es)) H3 1) ; auto ; try lia.
-  generalize (nthopt_preserves_wf _ _ H0 _ _ e1). intros.
-  generalize (cps_kvar_closed _ _ H5). intro.
-  apply (val_weaken _ _ _ H6 0 1).
-  (* Cons case *)
-  inversion H1 ; subst ; clear H1.
-  rewrite H ; auto.
-  Focus 2.
-  constructor.
-  apply (proj1 (proj1 (proj2 cps_kvar_closed') 0 es H8) 1).
-  repeat constructor.
-  generalize (val_weaken _ _ _ H2 0 (1 + N.of_nat(length es))).
-  replace (1 + N.of_nat(length es) + 0) with (1 + N.of_nat(length es)) ; try lia. auto.
-  rewrite vals_wf_append. split.
-  generalize (vals_weaken _ _ _ H3 0 (1 + N.of_nat(length es))).
-  replace (1 + N.of_nat(length es) + 0) with (1 + N.of_nat(length es)) ; try lia. auto.
-  repeat constructor. lia. apply wf_list_to_indices.
-  rewrite cps_val. Focus 2. eapply eval_yields_value ; eauto.
-  rewrite eval_ret. simpl.
-  rewrite eval_ret. simpl.
-  rewrite (ksubst_closed_val 0 0) ; try lia.
-  Focus 2. eapply cps_val_kvar_closed ; eauto. eapply (eval_preserves_wf) ; eauto.
-  rewrite cps_kshift_0.
-  rewrite ksubst_cps_cvts2 ; auto.
-  simpl. rewrite (ksubst_closed_val 0 0) ; eauto ; try lia.
-  fold ksubst_vals cps_cvt_vals. 
-  rewrite ksubst_vals_append.
-  erewrite ksubst_closed_vals ; eauto ; try lia. simpl.
-  repeat if_split.
-  rewrite kshift_closed_val ; eauto.
-  Focus 2. eapply cps_val_kvar_closed ; eauto. eapply eval_preserves_wf ; eauto.
-  rewrite ksubst_gt_indices ; try lia.
-  specialize (H0 H8 d k (ws ++ [cps_cvt_val v]) H2).
-  assert (vals_wf 0 0 (ws ++ [cps_cvt_val v])).
-  rewrite vals_wf_append. split ; auto. constructor.
-  eapply cps_val_kvar_closed ; eauto. eapply (eval_preserves_wf) ; eauto. constructor.
-  specialize (H0 H1 v').
-  rewrite <- app_assoc in H0. simpl in H0. rewrite H0.
-  rewrite (ksubst_closed_val 0 0) ; try lia ; auto.
-  rewrite ksubst_vals_append.
-  rewrite (ksubst_closed_vals 0 0) ; try lia ; auto. simpl.
-  repeat if_split. rewrite kshift_closed_val.
-  Focus 2. eapply cps_val_kvar_closed ; eauto. eapply eval_preserves_wf ; eauto.
-  rewrite ksubst_gt_indices ; try lia.
-  rewrite <- app_assoc. tauto.
-  Grab Existential Variables.
-  apply (cps_kvar_closed) ; eauto.
-  apply (cps_kvar_closed) ; eauto.
-  apply (cps_kvar_closed) ; eauto.
+  rewrite (fun l => proj2 (ball_true l));
+    [reflexivity|].
+  intros ?. simpl.
+  rewrite map_map. unfold compose. simpl.
+  intros Hin. apply in_map_iff in Hin. exrepnd. subst.
+  apply is_valueb_corr. eauto.
 Qed.
 
-Lemma cps_cvt_prog_corr :
-  forall e v, exp_wf 0 e -> eval e v -> eval_c (cps_cvt_prog e) (cps_cvt_val v).
+
+
+Lemma lsubstRet_c : forall sub a b, 
+  sub_range_sat sub closed
+  -> lsubst (Ret_c a b) sub = Ret_c (lsubst a sub) (lsubst b sub).
 Proof.
-  intros. unfold cps_cvt_prog.
-  rewrite (proj1 cps_cvt_corr e v H0 H) ; [idtac | repeat constructor ; auto ; lia].
-  rewrite (cps_val _ (eval_yields_value _ _ H0)).
-  rewrite eval_ret. simpl. rewrite eval_ret. simpl.
-  rewrite (ksubst_closed_val 0 0) ; try lia. Focus 2.
-  eapply cps_val_kvar_closed ; eauto. eapply eval_preserves_wf ; eauto.
-  rewrite val_kshift_0. constructor.
+  intros.
+  change_to_lsubst_aux4.
+  simpl. autorewrite with SquiggleLazyEq.
+  reflexivity.
 Qed.
 
-Lemma kshift_twice :
-  (forall c i j m n, i <= j -> j <= i + m -> kshift_cps n j (kshift_cps m i c) = kshift_cps (m+n) i c) /\
-  (forall v i j m n, i <= j -> j <= i + m -> kshift_val n j (kshift_val m i v) = kshift_val (m+n) i v) /\
-  (forall vs i j m n, i <= j -> j <= i + m -> kshift_vals n j (kshift_vals m i vs) = kshift_vals (m+n) i vs) /\
-  (forall bs i j m n, i <= j -> j <= i + m -> kshift_branches n j (kshift_branches m i bs) = kshift_branches (m+n) i bs) /\
-  (forall fs i j m n, i <= j -> j <= i + m -> kshift_fn_list n j (kshift_fn_list m i fs) = kshift_fn_list (m+n) i fs).
+Lemma lsubstKlam_c : forall sub x b, 
+  sub_range_sat sub closed
+  -> disjoint [x] (dom_sub sub)
+  -> lsubst (KLam_c x b) sub = KLam_c x (lsubst b sub).
 Proof.
-  Opaque N.add.
-  apply my_cps_ind ; simpl ; intros ; auto ;
-  try (rewrite H ; auto ; rewrite H0 ; auto ; rewrite H1 ; auto ; fail).
-  repeat if_split ; auto. replace (n + (m + n0)) with (n + m + n0) ; try lia ; auto.
-  rewrite (H (1+i) (1+j)) ; auto ; try lia.
-  rewrite (H (1+i) (1+j)) ; auto ; try lia.
-  rewrite (H (1+i) (1+j)) ; auto ; try lia.
-  rewrite H0 ; auto.
+  intros.
+  change_to_lsubst_aux4.
+  simpl. rewrite sub_filter_disjoint1;[| disjoint_reasoningv].
+  reflexivity.
 Qed.
 
-Lemma ushift_twice :
-  (forall c i j m n, i <= j -> j <= i + m -> ushift_cps n j (ushift_cps m i c) = ushift_cps (m+n) i c) /\
-  (forall v i j m n, i <= j -> j <= i + m -> ushift_val n j (ushift_val m i v) = ushift_val (m+n) i v) /\
-  (forall vs i j m n, i <= j -> j <= i + m -> ushift_vals n j (ushift_vals m i vs) = ushift_vals (m+n) i vs) /\
-  (forall bs i j m n, i <= j -> j <= i + m -> ushift_branches n j (ushift_branches m i bs) = ushift_branches (m+n) i bs) /\
-  (forall fs i j m n, i <= j -> j <= i + m -> ushift_fn_list n j (ushift_fn_list m i fs) = ushift_fn_list (m+n) i fs).
+Lemma substKlam_cTrivial : forall x (b t : CTerm),
+  closed t
+  -> lsubst (KLam_c x b) [(x,t)] = KLam_c x b.
 Proof.
-  apply my_cps_ind ; simpl ; intros ; auto ;
-  try (rewrite H ; auto ; rewrite H0 ; auto ; rewrite H1 ; auto ; fail).
-  repeat if_split ; auto. replace (n + (m + n0)) with (n + m + n0) ; try lia ; auto.
-  rewrite (H (1+i) (1+j)) ; auto ; try lia.
-  rewrite (H (n+i) (n+j)) ; auto ; try lia. rewrite H0 ; auto ; try lia.
-  rewrite (H (2+i) (2+j)) ; auto ; try lia.
-  rewrite H0 ; auto.
+  intros ? ? ? H.
+  change_to_lsubst_aux4;[ |simpl; rewrite H; disjoint_reasoningv; tauto].
+  simpl. rewrite memvar_singleton. rewrite <- beq_var_refl.
+  simpl. rewrite lsubst_aux_nil.
+  reflexivity.
 Qed.
 
-Lemma kshift_ushift_comm :
-  (forall c i j k l, kshift_cps i j (ushift_cps k l c) = ushift_cps k l (kshift_cps i j c)) /\
-  (forall v i j k l, kshift_val i j (ushift_val k l v) = ushift_val k l (kshift_val i j v)) /\
-  (forall vs i j k l, kshift_vals i j (ushift_vals k l vs) = ushift_vals k l (kshift_vals i j vs)) /\
-  (forall bs i j k l, kshift_branches i j (ushift_branches k l bs) = ushift_branches k l (kshift_branches i j bs)) /\
-  (forall fs i j k l, kshift_fn_list i j (ushift_fn_list k l fs) = ushift_fn_list k l (kshift_fn_list i j fs)).
+
+Lemma substKlam_cTrivial2 : forall x xx (b t : CTerm),
+  closed t
+  -> closed (KLam_c x b)
+  -> lsubst (KLam_c x b) [(xx,t)] = KLam_c x b.
 Proof.
-  apply my_cps_ind ; simpl ; intros ; auto ;
-  try (rewrite H ; auto ; rewrite H0 ; auto ; rewrite H1 ; auto ; fail) ; if_split.
+  intros ? ? ? ? H Hb.
+  change_to_lsubst_aux4;[ |simpl; rewrite H; disjoint_reasoningv; tauto].
+  simpl. rewrite memvar_singleton.
+  rewrite beq_deq. cases_if.
+  - simpl. rewrite lsubst_aux_nil.
+    reflexivity.
+  - unfold KLam_c. do 3 f_equal.
+    apply lsubst_aux_trivial_cl.
+    intros ? ? Hin. in_reasoning. inverts Hin.
+    split; [assumption|].
+    unfold closed in Hb. simpl in Hb.
+    autorewrite with core list in Hb.
+    rw nil_remove_nvars_iff in Hb.
+    firstorder.
 Qed.
 
-Lemma kshift_ksubst :
-  (forall c i k j v, k <= j -> kshift_cps i k (c[j:=v]) = (kshift_cps i k c)[j+i:=v]) /\
-  (forall w i k j v, k <= j -> kshift_val i k (w[j:=v]) = (kshift_val i k w)[j+i:=v]) /\
-  (forall ws i k j v, k <= j -> kshift_vals i k (ws[j:=v]) = (kshift_vals i k ws)[j+i:=v]) /\
-  (forall bs i k j v, k <= j -> kshift_branches i k (bs[j:=v]) = (kshift_branches i k bs)[j+i:=v]) /\
-  (forall fs i k j v, k <= j -> kshift_fn_list i k (fs[j:=v]) = (kshift_fn_list i k fs)[j+i:=v]).
+Lemma lsubstCall_c : forall sub a b d, 
+  sub_range_sat sub closed
+  -> lsubst (Call_c a b d) sub = Call_c (lsubst a sub) (lsubst b sub) (lsubst d sub).
 Proof.
-  apply my_cps_ind ; simpl ; intros ; auto ;
-  try (rewrite H ; auto ; rewrite H0 ; auto; rewrite H1 ; auto ; fail).
-  repeat if_split ; auto. destruct (lt_dec j k) ; auto. rewrite (proj1 (proj2 kshift_twice)) ;
-    auto ; try lia. rewrite (proj1 (proj2 kshift_twice)) ; auto ; try lia.
-  destruct (lt_dec n k) ; try lia. apply f_equal ; lia.
-  rewrite (H i (1 + k) (1 +j)). replace (1 + j + i) with (1 + (j + i)) ; try lia. auto. lia.
-  rewrite (H i (1 + k) (1 + j)). replace (1 + j + i) with (1 + (j + i)) ; try lia. auto. lia.
-  rewrite (H i (1 + k) (1 + j)) ; try lia. rewrite H0 ; try lia.
-  replace (1 + j + i) with (1 + (j + i)) ; auto ; try lia.
+  intros.
+  change_to_lsubst_aux4.
+  simpl. autorewrite with SquiggleLazyEq.
+  reflexivity.
 Qed.
 
-Lemma ushift_usubst :
-  (forall c i k j v, k <= j -> ushift_cps i k (c{j:=v}) = (ushift_cps i k c){j+i:=v}) /\
-  (forall w i k j v, k <= j -> ushift_val i k (w{j:=v}) = (ushift_val i k w){j+i:=v}) /\
-  (forall ws i k j v, k <= j -> ushift_vals i k (ws{j:=v}) = (ushift_vals i k ws){j+i:=v}) /\
-  (forall bs i k j v, k <= j -> ushift_branches i k (bs{j:=v}) = (ushift_branches i k bs){j+i:=v}) /\
-  (forall fs i k j v, k <= j -> ushift_fn_list i k (fs{j:=v}) = (ushift_fn_list i k fs){j+i:=v}).
-Proof.
-  apply my_cps_ind ; simpl ; intros ; auto ;
-  try (rewrite H ; auto ; rewrite H0 ; auto; rewrite H1 ; auto ; fail).
-  repeat if_split ; auto. destruct (lt_dec j k) ; auto. try lia.
-  rewrite (proj1 (proj2 ushift_twice)) ;
-    auto ; try lia. destruct (lt_dec n k) ; try lia. apply f_equal ; lia.
-  rewrite (H i (1 + k) (1 +j)). replace (1 + j + i) with (1 + (j + i)) ; try lia. auto. lia.
-  rewrite (H i (n + k) (n + j)). replace (n + j + i) with (n + (j + i)) ; try lia.
-  rewrite H0 ; auto. lia.
-  rewrite (H i (2 + k) (2 + j)) ; try lia. rewrite H0 ; try lia.
-  replace (2 + j + i) with (2 + (j + i)) ; auto ; try lia.
-Qed.
-
-(*
-Lemma kshift_usubst :
-  (forall c i k j v, k <= j -> kshift_cps i k (c{j:=v}) = (kshift_cps i k c){j:=kshift_val i k v}) /\
-  (forall w i k j v, k <= j -> kshift_val i k (w{j:=v}) = (kshift_val i k w){j:=kshift_val i k v}) /\
-  (forall ws i k j v, k <= j -> kshift_vals i k (ws{j:=v}) = (kshift_vals i k ws){j:=kshift_val i k v}) /\
-  (forall bs i k j v, k <= j -> kshift_branches i k (bs{j:=v}) = (kshift_branches i k bs){j:=kshift_val i k v}) /\
-  (forall fs i k j v, k <= j -> kshift_fn_list i k (fs{j:=v}) = (kshift_fn_list i k fs){j:=kshift_val i k v}).
-Proof.
-  apply my_cps_ind ; simpl ; intros ; auto ;
-  try (rewrite H ; auto ; rewrite H0 ; auto ; rewrite H1 ; auto ; fail).
-  repeat if_split. rewrite (proj1 (proj2 kshift_ushift_comm)). auto.
-*)
-  
-
-Lemma kshift_away_subst :
-  (forall c k i j v, k <= i -> i < k + (j + 1) ->
-        (kshift_cps (1+j) k c)[i:=v] = kshift_cps j k c) /\
-  (forall w k i j v, k <= i -> i < k + (j + 1) ->
-        (kshift_val (1+j) k w)[i:=v] = kshift_val j k w) /\
-  (forall ws k i j v, k <= i -> i < k + (j + 1) ->
-        (kshift_vals (1+j) k ws)[i:=v] = kshift_vals j k ws) /\
-  (forall bs k i j v, k <= i -> i < k + (j + 1) ->
-        (kshift_branches (1+j) k bs)[i:=v] = kshift_branches j k bs) /\
-  (forall fs k i j v, k <= i -> i < k + (j + 1) ->
-        (kshift_fn_list (1+j) k fs)[i:=v] = kshift_fn_list j k fs).
-Proof.
-  apply my_cps_ind ; simpl ; intros ; auto ;
-  try (rewrite H ; auto ; rewrite H0 ; auto ; rewrite H1 ; auto ; fail).
-  repeat if_split. apply f_equal. lia.
-  rewrite (H (1+k) (1+i)) ; try lia ; auto.
-  rewrite (H (1+k) (1+i)) ; try lia ; auto.
-  rewrite (H (1+k) (1+i)) ; try lia. rewrite H0 ; auto.
-Qed.
-
-Lemma ushift_away_subst :
-  (forall c k i j v, k <= i -> i < k + (j + 1) ->
-                     (ushift_cps (1+j) k c){i:=v} = ushift_cps j k c) /\
-  (forall w k i j v, k <= i -> i < k + (j + 1) ->
-                     (ushift_val (1+j) k w){i:=v} = ushift_val j k w) /\
-  (forall ws k i j v, k <= i -> i < k + (j + 1) ->
-                     (ushift_vals (1+j) k ws){i:=v} = ushift_vals j k ws) /\
-  (forall bs k i j v, k <= i -> i < k + (j + 1) ->
-                     (ushift_branches (1+j) k bs){i:=v} =
-                     ushift_branches j k bs) /\
-  (forall fs k i j v, k <= i -> i < k + (j + 1) ->
-                     (ushift_fn_list (1+j) k fs){i:=v} =
-                     ushift_fn_list j k fs).
-Proof.
-  apply my_cps_ind ; simpl ; intros ; auto ;
-  try (rewrite H ; auto ; rewrite H0 ; auto ; rewrite H1 ; auto ; fail).
-  repeat if_split. apply f_equal. lia.
-  rewrite (H (1+k) (1+i)) ; try lia ; auto.
-  rewrite (H (n+k) (n+i)) ; try lia. rewrite H0 ; auto.
-  rewrite (H (2+k) (2+i)) ; try lia. rewrite H0 ; auto.
-Qed.
-
-Lemma ksubst_comm :
-  (forall (c:cps) v1 v2 i j, i <= j -> c[i:=v1][j:=v2] = c[1+j:=v2][i:=v1[j-i:=v2]]) /\
-  (forall (w:val_c) v1 v2 i j, i <= j -> w[i:=v1][j:=v2] = w[1+j:=v2][i:=v1[j-i:=v2]]) /\
-  (forall (ws:list val_c) v1 v2 i j, i <= j -> ws[i:=v1][j:=v2] = ws[1+j:=v2][i:=v1[j-i:=v2]]) /\
-  (forall (bs:list (branch cps)) v1 v2 i j,
-     i <= j -> bs[i:=v1][j:=v2] = bs[1+j:=v2][i:=v1[j-i:=v2]]) /\
-  (forall (fs:list cps) v1 v2 i j, i <= j -> fs[i:=v1][j:=v2] = fs[1+j:=v2][i:=v1[j-i:=v2]]).
-Proof.
-  apply my_cps_ind ; simpl ; intros ; auto ;
-  try (rewrite H ; auto ; rewrite H0 ; auto ; rewrite H1 ; auto ; fail).
-  repeat if_split. generalize (proj1 (proj2 kshift_ksubst) v1 i 0 (j - i) v2).
-  unfold ksubstitute ; simpl. intros. rewrite H0 ; try lia.
-  replace (j - i + i) with j ; try lia ; auto.
-  generalize (proj1 (proj2 kshift_away_subst) v2 0 i (n-1)). unfold ksubstitute ; simpl.
-  intros. rewrite H0 ; try lia ; auto.
-  rewrite (H _ _ (1+i) (1+j)). replace (1 + j - (1 + i)) with (j - i) ; try lia ; auto. lia.
-  rewrite (H _ _ (1+i) (1+j)). replace (1 + j - (1 + i)) with (j - i) ; try lia ; auto. lia.
-  rewrite (H _ _ (1+i) (1+j)). replace (1 + j - (1 + i)) with (j - i) ; try lia ; auto.
-  rewrite H0 ; try lia. auto. lia.
-Qed.
-
-Lemma usubst_comm :
-  (forall (c:cps) v1 v2 i j, i <= j ->
-     c{i:=v1}{j:=v2} = c{1+j:=v2}{i:=v1{j-i:=v2}}) /\
-  (forall (w:val_c) v1 v2 i j, i <= j -> 
-     w{i:=v1}{j:=v2} = w{1+j:=v2}{i:=v1{j-i:=v2}}) /\
-  (forall (ws:list val_c) v1 v2 i j, i <= j -> 
-     ws{i:=v1}{j:=v2} = ws{1+j:=v2}{i:=v1{j-i:=v2}}) /\
-  (forall (bs:list (branch cps)) v1 v2 i j, i <= j -> 
-     bs{i:=v1}{j:=v2} = bs{1+j:=v2}{i:=v1{j-i:=v2}}) /\
-  (forall (fs:list cps) v1 v2 i j, i <= j ->
-     fs{i:=v1}{j:=v2} = fs{1+j:=v2}{i:=v1{j-i:=v2}}).
-Proof.
-  apply my_cps_ind ; simpl ; intros ; auto ;
-  try (rewrite H ; auto ; rewrite H0 ; auto ; rewrite H1 ; auto ; fail).
-  repeat if_split. generalize (proj1 (proj2 ushift_usubst) v1 i 0 (j - i) v2).
-  unfold substitute ; simpl. intros. rewrite H0 ; try lia.
-  replace (j - i + i) with j ; try lia ; auto.
-  generalize (proj1 (proj2 ushift_away_subst) v2 0 i (n-1)). unfold substitute ; simpl.
-  intros. rewrite H0 ; try lia ; auto.
-  rewrite (H _ _ (1+i) (1+j)) ; try lia.
-  replace (1 + j - (1 + i)) with (j - i) ; try lia ; auto.
-  rewrite (H _ _ (n+i) (n+j)) ; try lia.
-  replace (n + j - (n + i)) with (j - i) ; try lia ; auto. 
-  rewrite H0 ; try lia. replace (1 + (n + j)) with (n + (1 + j)) ; try lia ; auto.
-  rewrite (H _ _ (2+i) (2+j)) ; try lia. rewrite H0 ; try lia.
-  replace (2 + j - (2 + i)) with (j - i) ; try lia.
-  replace (1 + (2 + j)) with (2 + (1 + j)) ; try lia ; auto.
-Qed.
-
-(*
-Lemma usubst_kshift_comm :
-  (forall c v i j k, (ushift_cps i k c)[j:=ushift_val i k v] = ushift_cps i k (c[j:=v])) /\
-  (forall w v i j k, (ushift_val i k w)[j:=ushift_val i k v] = ushift_val i k (w[j:=v])) /\
-  (forall ws v i j k, (ushift_vals i k ws)[j:=ushift_val i k v] = ushift_vals i k (ws[j:=v])) /\
-  (forall bs v i j k, (ushift_branches i k bs)[j:=ushift_val i k v] = ushift_branches i k (bs[j:=v])) /\
-  (forall fs v i j k, (ushift_fn_list i k fs)[j:=ushift_val i k v] = ushift_fn_list i k (fs[j:=v])).
-Proof.
-  apply my_cps_ind ; simpl ; intros ; auto ;
-  try (rewrite H ; auto ; rewrite H0 ; auto ; rewrite H1 ; auto ; fail).
-  repeat if_split. apply (proj1 (proj2 kshift_ushift)).
-  rewrite <- (H v i (1 + j) (1 +k)).
-  Admitted.
-  
-Lemma uksubst_comm :
-  (forall (c:cps) v1 v2 i j, i <= j -> c{i:=v1}[j:=v2] = c[j:=v2]{i:=v1[j:=v2]}) /\
-  (forall (w:val_c) v1 v2 i j, i <= j -> w{i:=v1}[j:=v2] = w[j:=v2]{i:=v1[j:=v2]}) /\
-  (forall (ws:list val_c) v1 v2 i j, i <= j -> ws{i:=v1}[j:=v2] = ws[j:=v2]{i:=v1[j:=v2]}) /\
-  (forall (bs:list (branch cps)) v1 v2 i j, i <= j -> bs{i:=v1}[j:=v2] = bs[j:=v2]{i:=v1[j:=v2]}) /\
-  (forall (fs:list cps) v1 v2 i j, i <= j -> fs{i:=v1}[j:=v2] = fs[j:=v2]{i:=v1[j:=v2]}).
-Proof.
-  apply my_cps_ind ; simpl ; intros ; auto ;
-  try (rewrite H ; auto ; rewrite H0 ; auto ; rewrite H1 ; auto ; fail).
-  repeat if_split.
-*)
-  
-(** optimised cps reduction **)
-Inductive cps_red : cps -> cps -> Prop :=
-| reduce_ret_red :
-    forall c c' v v', val_red v v' -> cps_red c c' ->
-                      cps_red (Ret_c (Cont_c c) v) (c'[0:=v'])
-(*                                                             
-| reduce_call_red :
-    forall c c' v1 v1' v2 v2',
-      val_red v1 v1' -> val_red v2 v2' -> cps_red c c' ->
-      cps_red (Call_c (Lam_c c) v1 v2) (c'[0:=v1']{0:=v2'})
-| reduce_match_red :
-    forall d vs vs' bs c c',
-      find_branch d (N.of_nat (length vs)) bs = Some c ->
-      vals_red vs vs' -> 
-      cps_red c c' -> 
-      cps_red (Match_c (Con_c d vs) bs) (usubst_list c' vs')
-| reduce_proj_red :
-    forall cs n c c' v v',
-      nthopt (N.to_nat n) cs = Some c ->
-      val_red v v' -> 
-      cps_red c c' -> 
-      cps_red (Proj_c (Fix_c cs) n v) (Ret_c v' ((Lam_c c'){0:=Fix_c cs}))
-*)
-| halt_red :
-    forall v w, val_red v w -> cps_red (Halt_c v) (Halt_c w)
-| ret_red :
-    forall v1 v2 w1 w2, val_red v1 w1 -> val_red v2 w2 ->
-                        cps_red (Ret_c v1 v2) (Ret_c w1 w2)
-| call_red :
-    forall v1 v2 v3 w1 w2 w3,
-      val_red v1 w1 -> val_red v2 w2 -> val_red v3 w3 ->
-      cps_red (Call_c v1 v2 v3) (Call_c w1 w2 w3)
-| match_red :
-    forall v1 bs1 v2 bs2,
-      val_red v1 v2 -> branches_red bs1 bs2 ->
-      cps_red (Match_c v1 bs1) (Match_c v2 bs2)
-| proj_red :
-    forall v1 v2 n1 w1 w2 n2,
-      n1 = n2 -> val_red v1 w1 -> val_red v2 w2 ->
-      cps_red (Proj_c v1 n1 v2) (Proj_c w1 n2 w2)
-with val_red : val_c -> val_c -> Prop :=
-| var_red : forall n1 n2, n1 = n2 -> val_red (Var_c n1) (Var_c n2)
-| kvar_red : forall n1 n2, n1 = n2 -> val_red (KVar_c n1) (KVar_c n2)
-| lam_red : forall c1 c2, cps_red c1 c2 -> val_red (Lam_c c1) (Lam_c c2)
-| cont_red : forall c1 c2, cps_red c1 c2 -> val_red (Cont_c c1) (Cont_c c2)
-| con_red : forall d1 vs1 d2 vs2,
-             d1 = d2 -> vals_red vs1 vs2 ->
-             val_red (Con_c d1 vs1) (Con_c d2 vs2)
-| fix_red : forall cs1 cs2, fn_list_red cs1 cs2 ->
-                            val_red (Fix_c cs1) (Fix_c cs2)
-with vals_red : list val_c -> list val_c -> Prop :=
-| vals_nil_red : vals_red nil nil
-| vals_cons_red : forall v1 v1s v2 v2s,
-                   val_red v1 v2 -> vals_red v1s v2s ->
-                   vals_red (v1::v1s) (v2::v2s)
-with branches_red : list (branch cps) -> list (branch cps) -> Prop :=
-     | br_nil_red : branches_red nil nil
-     | br_cons_red : forall d1 n1 c1 bs1 d2 n2 c2 bs2,
-                      d1 = d2 -> n1 = n2 -> cps_red c1 c2 ->
-                      branches_red bs1 bs2 -> 
-                      branches_red ((d1,n1,c1)::bs1) ((d2,n2,c2)::bs2)
-with fn_list_red : list cps -> list cps -> Prop :=
-| fn_nil_red : fn_list_red nil nil
-| fn_cons_red : forall c1 c2 cs1 cs2,
-                 cps_red c1 c2 -> fn_list_red cs1 cs2 ->
-                 fn_list_red (c1::cs1) (c2::cs2).
-Hint Constructors fn_list_red vals_red branches_red val_red cps_red.
-Scheme cps_red_ind2 := Induction for cps_red Sort Prop
-with val_red_ind2 := Induction for val_red Sort Prop
-with vals_red_ind2 := Induction for vals_red Sort Prop
-with branches_red_ind2 := Induction for branches_red Sort Prop
-with fn_list_red_ind2 := Induction for fn_list_red Sort Prop.
-Combined Scheme my_cps_red_ind from cps_red_ind2, val_red_ind2,
-                vals_red_ind2, branches_red_ind2, fn_list_red_ind2.
-
-Lemma cps_red_refl' :
-  (forall c, cps_red c c) /\
-  (forall v, val_red v v) /\
-  (forall vs, vals_red vs vs) /\
-  (forall bs, branches_red bs bs) /\
-  (forall fs, fn_list_red fs fs).
-Proof.
-  apply my_cps_ind ; intros ; eauto.
-Qed.
-Definition cps_red_refl := proj1 cps_red_refl'.
-Definition val_red_refl := proj1 (proj2 cps_red_refl').
-Definition vals_red_refl := proj1 (proj2 (proj2 cps_red_refl')).
-Definition branches_red_refl := proj1 (proj2 (proj2 (proj2 cps_red_refl'))).
-Definition fn_list_red_refl := proj2 (proj2 (proj2 (proj2 cps_red_refl'))).
-Hint Resolve val_red_refl cps_red_refl vals_red_refl
-     branches_red_refl fn_list_red_refl.
-
-(** unoptimised cps reduction **)
-Inductive cps_ured : cps -> cps -> Prop :=
-| reduce_ret_ured :
-    forall c c' v v', val_ured v v' -> cps_ured c c' ->
-                      cps_ured (Ret_c (Cont_c c) v) (c'[0::=v'])
-| halt_ured :
-    forall v w, val_ured v w -> cps_ured (Halt_c v) (Halt_c w)
-| ret_ured :
-    forall v1 v2 w1 w2, val_ured v1 w1 -> val_ured v2 w2 ->
-                        cps_ured (Ret_c v1 v2) (Ret_c w1 w2)
-| call_ured :
-    forall v1 v2 v3 w1 w2 w3,
-      val_ured v1 w1 -> val_ured v2 w2 -> val_ured v3 w3 ->
-      cps_ured (Call_c v1 v2 v3) (Call_c w1 w2 w3)
-| match_ured :
-    forall v1 bs1 v2 bs2,
-      val_ured v1 v2 -> branches_ured bs1 bs2 ->
-      cps_ured (Match_c v1 bs1) (Match_c v2 bs2)
-| proj_ured :
-    forall v1 v2 n1 w1 w2 n2,
-      n1 = n2 -> val_ured v1 w1 -> val_ured v2 w2 ->
-      cps_ured (Proj_c v1 n1 v2) (Proj_c w1 n2 w2)
-with val_ured : val_c -> val_c -> Prop :=
-| var_ured : forall n1 n2, n1 = n2 -> val_ured (Var_c n1) (Var_c n2)
-| kvar_ured : forall n1 n2, n1 = n2 -> val_ured (KVar_c n1) (KVar_c n2)
-| lam_ured : forall c1 c2, cps_ured c1 c2 -> val_ured (Lam_c c1) (Lam_c c2)
-| cont_ured : forall c1 c2, cps_ured c1 c2 -> val_ured (Cont_c c1) (Cont_c c2)
-| con_ured : forall d1 vs1 d2 vs2,
-             d1 = d2 -> vals_ured vs1 vs2 ->
-             val_ured (Con_c d1 vs1) (Con_c d2 vs2)
-| fix_ured : forall cs1 cs2, fn_list_ured cs1 cs2 ->
-                            val_ured (Fix_c cs1) (Fix_c cs2)
-with vals_ured : list val_c -> list val_c -> Prop :=
-| vals_nil_ured : vals_ured nil nil
-| vals_cons_ured : forall v1 v1s v2 v2s,
-                   val_ured v1 v2 -> vals_ured v1s v2s ->
-                   vals_ured (v1::v1s) (v2::v2s)
-with branches_ured : list (branch cps) -> list (branch cps) -> Prop :=
-     | br_nil_ured : branches_ured nil nil
-     | br_cons_ured : forall d1 n1 c1 bs1 d2 n2 c2 bs2,
-                      d1 = d2 -> n1 = n2 -> cps_ured c1 c2 ->
-                      branches_ured bs1 bs2 -> 
-                      branches_ured ((d1,n1,c1)::bs1) ((d2,n2,c2)::bs2)
-with fn_list_ured : list cps -> list cps -> Prop :=
-| fn_nil_ured : fn_list_ured nil nil
-| fn_cons_ured : forall c1 c2 cs1 cs2,
-                 cps_ured c1 c2 -> fn_list_ured cs1 cs2 ->
-                 fn_list_ured (c1::cs1) (c2::cs2).
-Hint Constructors fn_list_ured vals_ured branches_ured val_ured cps_ured.
-Scheme cps_ured_ind2 := Induction for cps_ured Sort Prop
-with val_ured_ind2 := Induction for val_ured Sort Prop
-with vals_ured_ind2 := Induction for vals_ured Sort Prop
-with branches_ured_ind2 := Induction for branches_ured Sort Prop
-with fn_list_ured_ind2 := Induction for fn_list_ured Sort Prop.
-Combined Scheme my_cps_ured_ind from cps_ured_ind2, val_ured_ind2,
-                vals_ured_ind2, branches_ured_ind2, fn_list_ured_ind2.
-
-Lemma cps_ured_refl' :
-  (forall c, cps_ured c c) /\
-  (forall v, val_ured v v) /\
-  (forall vs, vals_ured vs vs) /\
-  (forall bs, branches_ured bs bs) /\
-  (forall fs, fn_list_ured fs fs).
-Proof.
-  apply my_cps_ind ; intros ; eauto.
-Qed.
-Definition cps_ured_refl := proj1 cps_ured_refl'.
-Definition val_ured_refl := proj1 (proj2 cps_ured_refl').
-Definition vals_ured_refl := proj1 (proj2 (proj2 cps_ured_refl')).
-Definition branches_ured_refl := proj1 (proj2 (proj2 (proj2 cps_ured_refl'))).
-Definition fn_list_ured_refl := proj2 (proj2 (proj2 (proj2 cps_ured_refl'))).
-Hint Resolve val_ured_refl cps_ured_refl vals_ured_refl
-     branches_ured_refl fn_list_ured_refl.
-
-(** optimised and unoptimised reduction relations are equivalent **)
-Lemma redc_uredc:
-  (forall c d:cps, cps_red c d -> cps_ured c d) /\
-  (forall v u:val_c, val_red v u -> val_ured v u) /\
-  (forall vs us, vals_red vs us -> vals_ured vs us) /\
-  (forall bs cs, branches_red bs cs -> branches_ured bs cs) /\
-  (forall bs cs, fn_list_red bs cs -> fn_list_ured bs cs).
-Proof.
-  apply my_cps_red_ind; simpl; intros; intuition.
-  - rewrite ksubst_ksbst_cps_0. constructor; assumption.
-Qed.
-
-Lemma kshft_pres_ured :
-  (forall c1 c2, cps_ured c1 c2 ->
-   forall j, cps_ured (kshft_cps j c1) (kshft_cps j c2)) /\
-  (forall v1 v2, val_ured v1 v2 ->
-   forall j, val_ured (kshft_val j v1) (kshft_val j v2)) /\
-  (forall vs1 vs2, vals_ured vs1 vs2 ->
-   forall j, vals_ured (kshft_vals j vs1) (kshft_vals j vs2)) /\
-  (forall bs1 bs2, branches_ured bs1 bs2 ->
-   forall j, branches_ured (kshft_branches j bs1) 
-                            (kshft_branches j bs2)) /\
-  (forall fs1 fs2, fn_list_ured fs1 fs2 ->
-   forall j, fn_list_ured (kshft_fn_list j fs1) (kshft_fn_list j fs2)).
-Proof.
-  apply my_cps_ured_ind; simpl; intros; subst; try constructor; intuition.
-  - change (cps_ured (Ret_c (Cont_c (kshft_cps (1 + j) c)) (kshft_val j v))
-     (kshft_cps j (c'[0::=v']))).
-    rewrite cps_kshft_ksbst. rewrite (N_i_plus_1 j).
-    apply (reduce_ret_ured _ _ _ _ (H j) (H0 (1+j))). lia.
-Qed.
-Definition cps_kshft_pres_ured := proj1 kshft_pres_ured.
-Definition val_kshft_pres_ured := proj1 (proj2 kshft_pres_ured).
-
-(**
-Lemma ushft_pres_ured :
-  (forall c1 c2, cps_ured c1 c2 ->
-   forall j, cps_ured (ushft_cps j c1) (ushft_cps j c2)) /\
-  (forall v1 v2, val_ured v1 v2 ->
-   forall j, val_ured (ushft_val j v1) (ushft_val j v2)) /\
-  (forall vs1 vs2, vals_ured vs1 vs2 ->
-   forall j, vals_ured (ushft_vals j vs1) (ushft_vals j vs2)) /\
-  (forall bs1 bs2, branches_ured bs1 bs2 ->
-   forall j, branches_ured (ushft_branches j bs1) (ushft_branches j bs2)) /\
-  (forall fs1 fs2, fn_list_ured fs1 fs2 ->
-   forall j, fn_list_ured (ushft_fn_list j fs1) (ushft_fn_list j fs2)).
-Proof.
-  apply my_cps_ured_ind; simpl; intros; subst; try constructor; intuition.
-  - change (cps_ured (Ret_c (Cont_c (ushft_cps j c)) (ushft_val j v))
-                     (ushft_cps j (c'[0::=v']))).
-
-    apply reduce_ret_ured. constructor.
-
-Lemma ushift_pres_ured :
-  (forall c1 c2, cps_ured c1 c2 ->
-   forall j n, cps_ured (ushift_cps j n c1) (ushift_cps j n c2)) /\
-  (forall v1 v2, val_ured v1 v2 ->
-   forall j n, val_ured (ushift_val j n v1) (ushift_val j n v2)) /\
-  (forall vs1 vs2, vals_ured vs1 vs2 ->
-   forall j n, vals_ured (ushift_vals j n vs1) (ushift_vals j n vs2)) /\
-  (forall bs1 bs2, branches_ured bs1 bs2 ->
-   forall j n, branches_ured (ushift_branches j n bs1) 
-                            (ushift_branches j n bs2)) /\
-  (forall fs1 fs2, fn_list_ured fs1 fs2 ->
-   forall j n, fn_list_ured (ushift_fn_list j n fs1) (ushift_fn_list j n fs2)).
-Proof.
-  apply my_cps_ured_ind; simpl; intros; subst; try constructor; intuition.
-  - change (cps_ured (Ret_c (Cont_c (ushift_cps j n c)) (ushift_val j n v))
-                     (ushift_cps j n (c'[0::=v']))).
-    apply reduce_ret_ured. constructor.
-
-  - change (cps_ured (Ret_c (Cont_c (ushift_cps (1 + j) c)) (ushift_val j v))
-     (ushift_cps j (c'[0::=v']))).
-    rewrite cps_ushift_ksbst. rewrite (N_i_plus_1 j).
-    apply (reduce_ret_ured _ _ _ _ (H j) (H0 (1+j))). lia.
-Qed.
-Definition cps_ushift_pres_ured := proj1 ushift_pres_ured.
-Definition val_ushift_pres_ured := proj1 (proj2 ushift_pres_ured).
-**)
-
-Lemma pre_uL1:  (** continuation variables **)
-  (forall c, forall v1 v2, val_ured v1 v2 ->
-     forall n, cps_ured (c[n ::= v1]) (c[n::= v2])) /\
-  (forall u, forall v1 v2, val_ured v1 v2 ->
-     forall n, val_ured (u[n ::= v1]) (u[n::= v2])) /\
-  (forall u, forall v1 v2, val_ured v1 v2 ->
-     forall n, vals_ured (u[n ::= v1]) (u[n::= v2])) /\
-  (forall u, forall v1 v2, val_ured v1 v2 ->
-     forall n, branches_ured (u[n ::= v1]) (u[n::= v2])) /\
-  (forall u, forall v1 v2, val_ured v1 v2 ->
-     forall n, fn_list_ured (u[n ::= v1]) (u[n::= v2])).
-Proof.
-  apply my_cps_ind; simpl; intros; intuition.
-  - if_split. destruct (N.eq_dec n n0).
-    + assumption.
-    + apply val_ured_refl.
-  - constructor. apply H. apply kshft_pres_ured. assumption.
-  - constructor. apply H. apply kshft_pres_ured. assumption.
-  - constructor.
-    + apply H. apply kshft_pres_ured. assumption.
-    + apply H0. assumption.
-Qed.
-Definition cps_pre_uL1 := proj1 pre_uL1.
-Definition val_pre_uL1 := proj1 (proj2 pre_uL1).
-
-Lemma uL1:  (** continuation variables **)
-  (forall c1 c2, cps_ured c1 c2 -> forall v1 v2, val_ured v1 v2 ->
-     forall n, cps_ured (c1[n ::= v1]) (c2[n::= v2])) /\
-  (forall u1 u2, val_ured u1 u2 -> forall v1 v2, val_ured v1 v2 ->
-     forall n, val_ured (u1[n ::= v1]) (u2[n::= v2])) /\
-  (forall u1 u2, vals_ured u1 u2 -> forall v1 v2, val_ured v1 v2 ->
-     forall n, vals_ured (u1[n ::= v1]) (u2[n::= v2])) /\
-  (forall u1 u2, branches_ured u1 u2 -> forall v1 v2, val_ured v1 v2 ->
-     forall n, branches_ured (u1[n ::= v1]) (u2[n::= v2])) /\
-  (forall u1 u2, fn_list_ured u1 u2 -> forall v1 v2, val_ured v1 v2 ->
-     forall n, fn_list_ured (u1[n ::= v1]) (u2[n::= v2])).
-Proof.
-  apply my_cps_ured_ind; simpl; intros; intuition.
-  - rewrite <- ksbst_ksbst_cps; try lia.
-    change (cps_ured
-     (Ret_c (Cont_c (c[1+n::=kshft_val 0 v1])) (v[n::= v1]))
-     ((c' [n + 1 ::= kshft_val 0 v2]) [0 ::= v' [n ::= v2]])).
-    apply (reduce_ret_ured (c[1+n::=kshft_val 0 v1])
-                           (c' [n + 1 ::= kshft_val 0 v2])).
-    + apply H. assumption.
-    + rewrite (N_i_plus_1). apply H0.
-      apply val_kshft_pres_ured. assumption.
-  - repeat if_split.
-  - constructor. apply H. apply val_kshft_pres_ured. assumption.
-  - constructor. apply H. apply val_kshft_pres_ured. assumption.
-  - constructor.
-    + apply H. apply val_kshft_pres_ured. assumption.
-    + apply H0. assumption.
-Qed.
-Definition cps_uL1 := proj1 uL1.
-Definition val_uL1 := proj1 (proj2 uL1).
-
-Lemma pre_UL1:  (** user variables **)
-  (forall c, forall v1 v2, val_ured v1 v2 ->
-     forall n, cps_ured (c{n ::= v1}) (c{n::= v2})) /\
-  (forall u, forall v1 v2, val_ured v1 v2 ->
-     forall n, val_ured (u{n ::= v1}) (u{n::= v2})) /\
-  (forall u, forall v1 v2, val_ured v1 v2 ->
-     forall n, vals_ured (u{n ::= v1}) (u{n::= v2})) /\
-  (forall u, forall v1 v2, val_ured v1 v2 ->
-     forall n, branches_ured (u{n ::= v1}) (u{n::= v2})) /\
-  (forall u, forall v1 v2, val_ured v1 v2 ->
-     forall n, fn_list_ured (u{n ::= v1}) (u{n::= v2})).
-Proof.
-  apply my_cps_ind; simpl; intros; intuition.
-  - if_split. destruct (N.eq_dec n n0).
-    + assumption.
-    + apply val_ured_refl.
-Qed.
-
-Lemma uL1:  (** user variables **)
-  (forall c1 c2, cps_ured c1 c2 -> forall v1 v2, val_ured v1 v2 ->
-     forall n, cps_ured (c1{n ::= v1}) (c2{n::= v2})) /\
-  (forall u1 u2, val_ured u1 u2 -> forall v1 v2, val_ured v1 v2 ->
-     forall n, val_ured (u1{n ::= v1}) (u2{n::= v2})) /\
-  (forall u1 u2, vals_ured u1 u2 -> forall v1 v2, val_ured v1 v2 ->
-     forall n, vals_ured (u1{n ::= v1}) (u2{n::= v2})) /\
-  (forall u1 u2, branches_ured u1 u2 -> forall v1 v2, val_ured v1 v2 ->
-     forall n, branches_ured (u1{n ::= v1}) (u2{n::= v2})) /\
-  (forall u1 u2, fn_list_ured u1 u2 -> forall v1 v2, val_ured v1 v2 ->
-     forall n, fn_list_ured (u1{n ::= v1}) (u2{n::= v2})).
-Proof.
-  apply my_cps_ured_ind; simpl; intros; intuition.
-  - rewrite <- ksbst_ksbst_cps; try lia.
-    change (cps_ured
-     (Ret_c (Cont_c (c{1+n::=kshft_val 0 v1})) (v{n::= v1}))
-     ((c' {n + 1 ::= kshft_val 0 v2}) {0 ::= v' {n ::= v2}})).
-    apply (reduce_ret_ured (c{1+n::=kshft_val 0 v1})
-                           (c' {n + 1 ::= kshft_val 0 v2})).
-    + apply H. assumption.
-    + rewrite (N_i_plus_1). apply H0.
-      apply val_kshft_pres_ured. assumption.
-  - repeat if_split.
-  - constructor. apply H. apply val_kshft_pres_ured. assumption.
-  - constructor. apply H. apply val_kshft_pres_ured. assumption.
-  - constructor.
-    + apply H. apply val_kshft_pres_ured. assumption.
-    + apply H0. assumption.
-Qed.
-Definition cps_uL1 := proj1 uL1.
-Definition val_uL1 := proj1 (proj2 uL1).
-
-Lemma cps_ured_sound :
-  forall c v, ueval_c c v -> forall c', cps_ured c c' ->
-    exists v', ueval_c c' v' /\ val_ured v v'.
-Proof.
-  induction 1 ; intros; assert (j:= val_ured_refl).
-  * inversion H ; subst ; eauto.
-  * inversion H0 ; subst ; clear H0.
-    apply IHueval_c. apply cps_uL1 ; auto.
-    inversion H3 ; clear H3 ; subst. Check (cps_uL1 _ _ H1 _ _ H5 _).
-    specialize (IHueval_c (c2 [0 ::= w2]) (cps_uL1 _ _ H1 _ _ H5 _)).
-    destruct IHueval_c as [w [H2 H3]]. eauto.
-  * inversion H0 ; subst. clear H0. inversion H4 ; subst. clear H4.
-    specialize (IHueval_c (c2[0::= w2]{0:=w3})).
-    Check (cps_uL1 _ _ H1).
-    destruct (IHueval_c _ (cps_uL1 _ _ H1 _ _ _ _)) as [w [H6 H7]] ; eauto.
-Check (cps_uL1 _ _ H1 _ _ H6).
-    apply (cps_uL1 _ _ H1 _ _ H6). cps_uL1 ; eauto.
-    inversion H3 ; subst ; clear H3.
-    destruct (IHeval_c _ (cps_red_ksubst _ _ H1 _ _ 0 H5)) as [w [H6 H7]] ; eauto
-Lemma cps_red_usound :
-  forall c v, ueval_c c v -> forall c', cps_ured c c' ->
-    exists v', ueval_c c' v' /\ val_ured v v'.
-Proof.
-  induction 1 ; intros.
-  * exists v. intuition. inversion H ; subst ; eauto.
-  * inversion H0 ; subst ; clear H0.
-    apply IHeval_c. apply cps_red_ksubst ; auto.
-    inversion H3 ; clear H3 ; subst.
-    specialize (IHeval_c (c2 [0 := w2]) (cps_red_ksubst _ _ H1 _ _ 0 H5)).
-    destruct IHeval_c as [w [H2 H3]]. eauto.
-  * inversion H0 ; clear H0 ; subst. inversion H4 ; clear H4 ; subst.
-    specialize (IHeval_c (c2[0:= w2]{0:=w3})).
-
-
-
-Goal
-  forall c v, ueval_c c v -> forall v', val_ured v v' -> 
-      exists c', cps_ured c c'.
-Proof.
-  induction 1; intros u h.
-  - exists (Halt_c u). constructor. assumption.
-  - 
-
-
-Lemma cps_red_usound :
-  forall c v, ueval_c c v -> forall c', cps_ured c c' ->
-    exists v', ueval_c c' v' /\ val_ured v v'.
-Proof.
-  induction 1 ; intros.
-  - inversion H; subst; clear H. exists w. intuition. constructor.
-  - inversion H0; subst; clear H0.
-    + apply IHueval_c. apply cps_uL1; assumption.
-    + inversion H3; subst; clear H3.
-      destruct (IHueval_c (c [0 ::= v]) (cps_ured_refl _)) as [x [j1 j2]].
-      exists x. intuition.
-      constructor. admit.
-  - inversion H0; subst; clear H0. inversion H4. subst.
-    inversion H4. subst. clear H4.
-    exists v'. split. apply (proj2 (ueval_call _ _ _ _)). admit. admit.
-  - inversion H1. subst. inversion H1. subst. clear H1. admit.
-  -  inversion H1. subst. 
-
-
-apply IHueval_c. 
-
-
-
-ksbst_pres_ueval
-ueval_single valued.
-
-
-    + inversion H; subst; clear H.
-
-apply IHueval_c. apply uL1; assumption.
-    + assert (j:= cps_ured (c [0 ::= v]) (c'0 [0 ::= v'0])).
-
-
-Require Import Relations.
-
-Definition cps_red_star := clos_refl_trans cps cps_red.
-Definition val_red_star := clos_refl_trans val_c val_red.
-Definition vals_red_star := clos_refl_trans (list val_c) vals_red.
-Definition branches_red_star := clos_refl_trans _ branches_red.
-Definition fn_list_red_star := clos_refl_trans _ fn_list_red.
-
-
-Lemma length_ksubst_vals :
-  forall v i vs, length (ksubst_vals v i vs) = length vs.
-Proof.
-  induction vs ; simpl ; intros ; auto.
-Qed.
-
-Lemma find_ksubst_branch :
-  forall d n bs c v i, 
-    find_branch d n bs = Some c ->
-    find_branch d n (ksubst_branches v i bs) = Some (ksubst_cps v i c).
-Proof.
-  induction bs ; simpl ; intros ; try discriminate. unfold ksubst_branch ; unfold br in *.
-  destruct a ; destruct p.
-  destruct (N.eq_dec d d0) ; destruct (N.eq_dec n0 n) ; try discriminate ; subst.
-  congruence. apply IHbs ; auto. apply IHbs ; auto.
-Qed.
-
-(*
-Lemma ksubst_usubst_comm' :
-  (forall (c:cps) v1 v2 i j, (c{i:=v1})[j:=v2] = (c[j:=v2]){i:=v1[j:=v2]}) /\
-  (forall (w:val_c) v1 v2 i j, w{i:=v1}[j:=v2] = w[j:=v2]{i:=v1[j:=v2]}) /\
-  (forall (ws:list val_c) v1 v2 i j, ws{i:=v1}[j:=v2] = ws[j:=v2]{i:=v1[j:=v2]}) /\
-  (forall (bs:list (branch cps)) v1 v2 i j, bs{i:=v1}[j:=v2] = bs[j:=v2]{i:=v1[j:=v2]}) /\
-  (forall (fs:list cps) v1 v2 i j, fs{i:=v1}[j:=v2] = fs[j:=v2]{i:=v1[j:=v2]}).
-Proof.
-  apply my_cps_ind ; simpl ; intros ; auto ;
-  try (rewrite H ; auto ; rewrite H0 ; auto ; rewrite H1 ; auto ; fail).
-  repeat if_split.
+(** derive it from a more general lemma, similar to [cps_cvt_aux_fvars] below *)
+Lemma cps_cvt_val_closed : forall e,
+  closed e
+  -> closed (cps_cvt_val e).
 Admitted.
 
-Lemma ksubst_usubst_list_comm :
-  forall vs i v c,
-    (usubst_list c vs)[i:=v] = usubst_list (c[i:=v]) (vs[i:=v]).
-Proof.
-  induction vs ; simpl in * ; intros ; auto.
-  rewrite IHvs. rewrite (proj1 ksubst_usubst_comm'). auto.
-Qed.
-*)
-
-Lemma nth_ksubst_fn_list :
-  forall n cs c v i,
-    nthopt n cs = Some c ->
-    nthopt n (ksubst_fn_list v i cs) = Some (ksubst_cps v (1+i) c).
-Proof.
-  induction n ; destruct cs ; simpl ; intros ; try discriminate. congruence.
-  apply IHn ; auto.
-Qed.
-
-(*
-Lemma ksubst_kshift2 :
-  (forall c i j k l v, ksubst_cps (kshift_val i j v) k (kshift_cps i (l+j) c) =
-                     kshift_cps i j (ksubst_cps v k c)) /\
-  (forall w i j k l v, ksubst_val (kshift_val i j v) k (kshift_val i (l+j) w) =
-                     kshift_val i j (ksubst_val v k w)) /\
-  (forall ws i j k l v, ksubst_vals (kshift_val i j v) k (kshift_vals i (l+j) ws) =
-                                 kshift_vals i j (ksubst_vals v k ws)) /\
-  (forall bs i j k l v, ksubst_branches (kshift_val i j v) k (kshift_branches i (l+j) bs) =
-                        kshift_branches i j (ksubst_branches v k bs)) /\
-  (forall fs i j k l v, ksubst_fn_list (kshift_val i j v) k (kshift_fn_list i (l+j) fs) =
-                      kshift_fn_list i j (ksubst_fn_list v k fs)).
-Proof.
-  apply my_cps_ind ; simpl ; intros ; auto.
-  rewrite H ; auto.
-  rewrite H ; rewrite H0 ; auto.
-  rewrite H ; rewrite H0 ; rewrite H1 ; auto.
-  rewrite H ; rewrite H0 ; auto.
-  rewrite H ; rewrite H0 ; auto.
-  Focus 2.
-  specialize (H i j (1+k) (1+l) v).
-  replace (1 + (l + j)) with (1 + l + j) ; try lia. rewrite H.
-  try (auto ; rewrite H ; auto ; rewrite H0 ; auto ; rewrite H1 ; auto ; fail).
-  repeat if_split.
-
-  (shift i l c)[k := (shift i j v)
-  Admitted.
-*)
-
-
-Lemma cps_red_ksubst' :
-  (forall c1 c2, cps_red c1 c2 ->
-   forall v1 v2 i, val_red v1 v2 -> cps_red (c1[i:=v1]) (c2[i:=v2])) /\
-  (forall w1 w2, val_red w1 w2 ->
-   forall v1 v2 i, val_red v1 v2 -> val_red (w1[i:=v1]) (w2[i:=v2])) /\
-  (forall ws1 ws2, vals_red ws1 ws2 ->
-   forall v1 v2 i, val_red v1 v2 -> vals_red (ws1[i:=v1]) (ws2[i:=v2])) /\
-  (forall bs1 bs2, branches_red bs1 bs2 ->
-   forall v1 v2 i, val_red v1 v2 -> branches_red (bs1[i:=v1]) (bs2[i:=v2])) /\
-  (forall fs1 fs2, fn_list_red fs1 fs2 ->
-   forall v1 v2 i, val_red v1 v2 -> fn_list_red (fs1[i:=v1]) (fs2[i:=v2])).
-Proof.
-  Opaque N.add.
-  apply my_cps_red_ind ; simpl in * ; intros ; eauto.
-  - rewrite (proj1 ksubst_comm) ; try lia.
-    replace (i - 0) with i ; try lia. eauto.
-  - subst. repeat if_split. apply cps_red_kshift ; auto.
-Qed.
-Definition cps_red_ksubst := proj1 cps_red_ksubst'.
-
-
-(*** 
-Lemma cps_red_ushift :
-  (forall c1 c2, cps_red c1 c2 ->
-                 forall i j, cps_red (ushift_cps i j c1) (ushift_cps i j c2)) /\
-  (forall v1 v2, val_red v1 v2 ->
-                 forall i j, val_red (ushift_val i j v1) (ushift_val i j v2)) /\
-  (forall vs1 vs2, vals_red vs1 vs2 ->
-                   forall i j, vals_red (ushift_vals i j vs1) (ushift_vals i j vs2)) /\
-  (forall bs1 bs2, branches_red bs1 bs2 ->
-                   forall i j, branches_red (ushift_branches i j bs1) (ushift_branches i j bs2)) /\
-  (forall fs1 fs2, fn_list_red fs1 fs2 ->
-                   forall i j, fn_list_red (ushift_fn_list i j fs1) (ushift_fn_list i j fs2)).
-Proof.
-  apply my_cps_red_ind ; intros ; subst ; simpl ; try (constructor ; eauto ; fail).
-  replace (ushift_cps i j (usubst_cps v' 0 c')) with (usubst_cps (ushift_val i j v') 0 (ushift_cps i (1+j) c')).
-  constructor ; eauto.
+Lemma cps_cvt_aux_fvars : forall e lv,
+  subsetv (free_vars e) lv ->
+  eqsetv (free_vars (cps_cvt_aux lv e)) (free_vars e).
 Admitted.
 
-Lemma cps_red_usubst' :
-  (forall c1 c2, cps_red c1 c2 ->
-                 forall v1 v2 i, val_red v1 v2 -> cps_red (c1{i:=v1}) (c2{i:=v2})) /\
-  (forall w1 w2, val_red w1 w2 ->
-                 forall v1 v2 i, val_red v1 v2 -> val_red (w1{i:=v1}) (w2{i:=v2})) /\
-  (forall ws1 ws2, vals_red ws1 ws2 ->
-                 forall v1 v2 i, val_red v1 v2 -> vals_red (ws1{i:=v1}) (ws2{i:=v2})) /\
-  (forall bs1 bs2, branches_red bs1 bs2 ->
-                 forall v1 v2 i, val_red v1 v2 -> branches_red (bs1{i:=v1}) (bs2{i:=v2})) /\
-  (forall fs1 fs2, fn_list_red fs1 fs2 ->
-                   forall v1 v2 i, val_red v1 v2 -> fn_list_red (fs1{i:=v1}) (fs2{i:=v2})).
+
+Lemma eval_c_subst_commute : forall x e1' v2,
+lsubst (cps_cvt_aux [x] e1') [(x, cps_cvt_val v2)]
+= cps_cvt_aux [] (lsubst e1' [(x, v2)]).
+Admitted.
+
+
+Lemma cps_cvt_corr : forall e v,
+  eval e v ->
+  closed e ->
+  forall k, closed k ->
+    forall v', 
+      eval_c (Ret_c (cps_cvt_aux [] e) k) v' <->
+        eval_c (Ret_c (cps_cvt_aux [] v) k) v'.
 Proof.
-  apply my_cps_red_ind ; simpl ; intros ; subst ; eauto.
-  Focus 2.
-  repeat if_split.
+  intros ? ? He. induction He; try (simpl ; tauto; fail);[| | | |].
+  (* application case *)
+- intros Hcle ? Hcl ?.
+   unfold App_e. simpl.
+  destruct (fresh_vars 3 []) as [kv Hflv]. simpl.
+  repnd.  dlist_len_name kv kv. simpl.
+  unfold closed in Hcle. simpl in Hcle.
+  autorewrite with core list in Hcle.
+  apply app_eq_nil in Hcle. repnd.
+  specialize (IHHe1 Hcle0).
+  specialize (IHHe2 Hcle).
+  pose proof (subsetv_step_app x e1' v2) as Hsss.
+  simpl in IHHe3. unfold subst in IHHe3.
+  applydup eval_reduces_fvars in He1 as Hss.
+  applydup eval_reduces_fvars in He2 as Hss2.
+  apply subsetv_prop in Hss.
+  apply subsetv_prop in Hss2.
+  rewrite Hcle0 in Hss. apply subsetv_nil_r in Hss.
+  rewrite Hcle in Hss2. apply subsetv_nil_r in Hss2.
+  simpl in Hss, Hsss.
+  autorewrite with list core in *.
+  dimp IHHe3;
+    [apply subsetv_nil_r; eapply transitivity;[apply Hsss|]; simpl; 
+      apply subsetv_app_l;
+     split;  apply subsetv_nil_r; eauto|].
+  specialize (IHHe3 hyp).
+  clear hyp.
+  rewrite <- IHHe3;[| assumption].
+
+  rewrite eval_ret.
+  simpl. unfold subst. 
+  assert (sub_range_sat [(kv0, k)] closed) as Hcs by
+    (intros ? ? ?; in_reasoning; cpx).
+  rewrite lsubstRet_c by assumption.
+  rewrite lsubstKlam_c; [| assumption| noRepDis].
+  rewrite lsubstRet_c by assumption.
+  rewrite lsubstKlam_c; [| assumption| noRepDis].
+  rewrite lsubstCall_c by assumption.
+  do 3 rewrite lsubst_vterm. simpl.
+  rewrite <- beq_var_refl.
+  rewrite not_eq_beq_var_false;[| noRepDis].
+  rewrite not_eq_beq_var_false;[| noRepDis].
+  rewrite lsubst_trivial3.
+  Focus 2. 
+    setoid_rewrite in_single_iff.
+    intros ? ? ?. cpx. rewrite Hcl.
+    split;[disjoint_reasoningv|].
+    rewrite cps_cvt_aux_fvars; rewrite Hcle0; [ tauto | eauto ].
+  rewrite lsubst_trivial3.
+  Focus 2. 
+    setoid_rewrite in_single_iff.
+    intros ? ? ?. cpx. rewrite Hcl.
+    split;[disjoint_reasoningv|].
+    rewrite cps_cvt_aux_fvars; rewrite Hcle; [ tauto | eauto ].
+    
+  clear Hcs.
+  match goal with
+  [|- context [Ret_c _ ?k]] => assert (closed k) as Hclk;
+    [|  assert (sub_range_sat [(fresh_var [] , k)] closed) as Hcs by
+        (intros ? ? ?; in_reasoning; cpx)]
+  end.
+    unfold closed. simpl. autorewrite with list core.
+    apply null_iff_nil.
+    rewrite cps_cvt_aux_fvars; rewrite Hcle; [  | eauto ].
+    apply null_iff_nil. simpl. rewrite Hcl. simpl.
+    unfold remove_nvars. simpl.
+    repeat match goal with
+    [ |- context [eq_var_dec ?a ?b] ] 
+      => destruct (eq_var_dec a b); simpl; [try reflexivity| try noRepDis]
+    end.
+
+  rewrite IHHe1; [| assumption]. simpl.
+  rewrite eval_ret. simpl.
+  unfold subst.
+  rewrite lsubstRet_c by assumption.
+  rewrite lsubst_vterm. simpl.
+  rename Hcs into Hcsss.
+  simpl. rename Hclk into Hclkk.
+  match goal with
+  [|- context [Ret_c _ (lsubst ?k _)]] => assert (closed k) as Hclk;
+    [|  assert (sub_range_sat [(kv1 , k)] closed) as Hcs by
+        (intros ? ? ?; in_reasoning; cpx)]
+  end.
+    unfold closed. simpl. autorewrite with list core.
+    apply null_iff_nil. pose proof Hss as Hssb.
+    apply null_iff_nil, null_remove_nvars_subsetv in Hss.
+    rewrite (cons_as_app _ x []).
+    rewrite cps_cvt_aux_fvars; [ | apply subsetv_app_weak_l; assumption].
+    apply null_iff_nil. simpl.
+    rewrite remove_nvars_app_r, Hssb. simpl.
+    rewrite remove_nvars_comm, remove_nvars_eq. reflexivity.
+
+  rewrite substKlam_cTrivial2 by  assumption.
+
+  rewrite eval_ret. simpl.
+  unfold subst.
+  rewrite lsubstRet_c by assumption.
+  rewrite lsubstKlam_c; [| assumption| noRepDis].
+  rewrite lsubstCall_c by assumption.
+  do 2 rewrite lsubst_vterm. simpl.
+  rewrite <- beq_var_refl.
+  rewrite not_eq_beq_var_false;[| noRepDis].
+  rewrite lsubst_trivial2_cl;[| assumption | 
+      apply null_iff_nil; rewrite cps_cvt_aux_fvars; rewrite Hcle; eauto].
+  rewrite lsubst_trivial2_cl;[| assumption | assumption].
+  clear Hcs.
+  rename Hclk into Hclkb.
+  match goal with
+  [|- context [Ret_c _ ?k]] => assert (closed k) as Hclk;
+    [|  assert (sub_range_sat [(fresh_var [] , k)] closed) as Hcs by
+        (intros ? ? ?; in_reasoning; cpx)]
+  end.
+    unfold closed.
+    match type of Hclkb with
+    closed ?k => remember k as kr
+    end.
+    simpl. autorewrite with list core.
+    rewrite Hclkb, Hcl. simpl.
+    rewrite remove_nvars_eq. reflexivity.
   
-Definition cps_red_usubst := proj1 cps_red_usubst'.
+  clear Hcs.
+  rewrite IHHe2 by assumption.
+  pose proof (cps_val v2 Hss2) as Hv.
+  simpl in Hv.
+  dimp Hv;[eauto using eval_yields_value'|].
+  clear Hv. rename hyp into Hv.
+  unfold cps_cvt in Hv.
+  rewrite Hss2 in Hv.
+  rewrite Hv. clear Hv.
+  rename Hclk into Hclk3b.
+  match goal with
+  [|- context [Ret_c _ ?k]] => assert (closed k) as Hclk;
+    [assumption |  assert (sub_range_sat [(fresh_var [] , k)] closed) as Hcs by
+        (intros ? ? ?; in_reasoning; cpx)]
+  end.
+  rewrite eval_ret. simpl. unfold subst.
+  rewrite lsubstRet_c by assumption.
+  rewrite lsubst_vterm. simpl.
+  assert (closed (cps_cvt_val v2)) as Hc2v by (auto using cps_cvt_val_closed).
+  rewrite lsubst_trivial2_cl;[| assumption | 
+    assumption
+      ].
+  clear Hcs.
+  match goal with
+  [|- context [Ret_c _ ?kk]] => 
+      assert (sub_range_sat [(kv2 , kk)] closed)
+       as Hcs by
+        (intros ? ? ?; in_reasoning; cpx)
+  end.
 
+  rewrite eval_ret.
+  simpl. unfold subst.
+  simpl.
+  rewrite lsubstCall_c by assumption.
+  rewrite lsubst_vterm. simpl.
+  rewrite <- beq_var_refl. simpl.
+  do 2 (rewrite lsubst_trivial2_cl;[| assumption | 
+    assumption
+      ]).
+  rewrite eval_call. simpl.
+  unfold subst.
+  do 2 (rewrite lsubstRet_c by 
+        (intros ? ? ?; in_reasoning; cpx)).
+  rewrite lsubst_trivial2_cl;[|
+     (intros ? ? ?; in_reasoning; cpx) | 
+      ].
+  Focus 2 .
+    unfold closed. rewrite fvars_lsubst1; simpl;
+      [| (intros ? ? ?; in_reasoning; cpx)].
+    apply null_iff_nil.
+    rewrite cps_cvt_aux_fvars;
+       [ apply null_iff_nil; assumption|].
+    apply null_remove_nvars_subsetv, null_iff_nil.
+    assumption.
+  rewrite lsubst_vterm.
+  simpl.
+  pose proof (fresh_var_not_in [x]) as Hf.
+  rewrite in_single_iff in Hf.
+  rewrite not_eq_beq_var_false;[| auto].
+  clear Hf.
+  rewrite lsubst_vterm. 
+  simpl. rewrite <- beq_var_refl.
+  rewrite eval_c_subst_commute.
+  reflexivity.
 
-Lemma cps_red_usubst_list :
-  forall v1s v2s, vals_red v1s v2s ->
-                forall c1 c2, cps_red c1 c2 -> cps_red (usubst_list c1 v1s) (usubst_list c2 v2s).
-Proof.
-  induction 1 ; simpl ; auto ; intros.
-  apply IHvals_red. apply cps_red_usubst ; auto.
-Qed.
-*)
+  (* constructor *)
+- admit.
+Abort.
 
-Lemma find_branch_pres_red :
-  forall bs1 bs2, branches_red bs1 bs2 ->
-    forall d n c1, find_branch d n bs1 = Some c1 ->
-      exists c2, (find_branch d n bs2 = Some c2 /\ cps_red c1 c2).
-Proof.
-  induction 1 ; simpl ; intros. discriminate.
-  subst. destruct (N.eq_dec d d2). subst.
-  destruct (N.eq_dec n2 n) ; try discriminate.
-  injection H3 ; intros ; subst. eauto.
-  apply IHbranches_red. auto.
-Qed.
-
-Lemma fn_list_pres_red :
-  forall n fs1 fs2, fn_list_red fs1 fs2 ->
-    forall c1, nthopt n fs1 = Some c1 ->
-      exists c2, (nthopt n fs2 = Some c2 /\ cps_red c1 c2).
-Proof.
-  induction n ; simpl in *; intros.
-  inversion H ; subst ; try discriminate ; clear H.
-  injection H0 ; intros ; subst. eauto.
-  inversion H ; subst ; try discriminate ; clear H.
-  apply (IHn _ _ H2 _ H0).
-Qed.
-
-Lemma fn_list_red_same_len :
-  forall fs1 fs2, fn_list_red fs1 fs2 -> length fs1 = length fs2.
-Proof.
-  induction 1 ; simpl ; intros ; subst ; auto.
-Qed.  
-  
-Lemma vals_red_same_len :
-  forall vs1 vs2, vals_red vs1 vs2 -> length vs1 = length vs2.
-Proof.
-  induction 1 ; simpl ; intros ; auto.
-Qed.
-
-
-
-Lemma cps_red_sound :
-  forall c v, eval_c c v -> forall c', cps_red c c' ->
-    exists v', eval_c c' v' /\ val_red v v'.
-Proof.
-  Hint Constructors eval_c.
-  induction 1 ; intros; assert (j:= val_red_refl)
-  * inversion H ; subst ; eauto.
-  * inversion H0 ; subst ; clear H0.
-    apply IHeval_c. apply cps_red_ksubst ; auto.
-    inversion H3 ; clear H3 ; subst.
-    specialize (IHeval_c (c2 [0 := w2]) (cps_red_ksubst _ _ H1 _ _ 0 H5)).
-    destruct IHeval_c as [w [H2 H3]]. eauto.
-  * inversion H0 ; clear H0 ; subst. inversion H4 ; clear H4 ; subst.
-    specialize (IHeval_c (c2[0:= w2]{0:=w3})).
-
-
-    apply cps_red_ksubst ; eauto.
-    inversion H3 ; subst ; clear H3.
-    destruct (IHeval_c _ (cps_red_ksubst _ _ H1 _ _ 0 H5)) as [w [H6 H7]] ; eauto.
-  * inversion H0 ; subst ; clear H0.
-    apply IHeval_c. apply cps_red_usubst ; eauto. apply cps_red_ksubst ; eauto.
-    inversion H4 ; subst ; clear H4.
-    specialize (cps_red_ksubst _ _ H1 _ _ 0 H6) ; intro.
-    specialize (cps_red_usubst _ _ H0 _ _ 0 H7) ; intro.
-    specialize (IHeval_c _ H2). destruct IHeval_c as [w [H8 H9]] ; eauto.
-  * inversion H1 ; clear H1 ; subst.
-    rewrite H in H5. injection H5 ; intros ; subst ; clear H5.
-    apply IHeval_c. eapply cps_red_usubst_list ; eauto.
-    inversion H4 ; subst ; clear H4.
-    destruct (find_branch_pres_red _ _ H6 _ _ _ H) as [c' [H8 H9]].
-    specialize (cps_red_usubst_list _ _ H7 _ _ H9). intro.
-    specialize (IHeval_c _ H1). destruct IHeval_c as [v [H10 H11]].
-    exists v. rewrite (vals_red_same_len _ _ H7) in H8. eauto.
-  * inversion H1 ; subst ; clear H1. rewrite H in H5.
-    injection H5 ; intros ; subst ; clear H5. apply IHeval_c.
-    apply ret_red ; auto. simpl. apply lam_red.
-    apply (cps_red_usubst _ _ H8 (Fix_c cs) _ 1 (val_red_refl _)). 
-    inversion H7 ; subst ; clear H7.
-    destruct (fn_list_pres_red _ _ _ H2 _ H) as [c' [H9 H10]].
-    assert (cps_red (Ret_c k ((Lam_c c) {0 := Fix_c cs}))
-                    (Ret_c w2 ((Lam_c c'){0 := Fix_c cs2}))).
-    constructor. auto. simpl. constructor ; auto.
-    eapply (cps_red_usubst) ; eauto.
-    specialize (IHeval_c _ H1). destruct IHeval_c as [v [H11 H12]].
-    exists v ; eauto.
-Qed.
-
-(* Todo:
-
-1. replace nat with positive or BinNat's [Done]
-2. Adam-ize
-   * introduce lemmas, hints to make proofs go through easier
-3. Add constructors  C(e1,...,en) [Done]
-4. Add pattern matching [Done]
-5. Add mutually recursive functions [Done]
-6. Add let to the source [Done]
-7. Relate to optimized translation -- 
-   requires setting up a Beta-value relation.
-
-*)*)
